getting better but it's getting too long

SubsetSum_DTM_Bridge.thy
@@ -2,17 +2,17 @@ theory SubsetSum_DTM_Bridge
   imports "SubsetSum_DecisionTree"
 begin
 
-section ‹DTM bridge: abstract run model›
+section \<open>DTM bridge: abstract run model\<close>
 
 fun wf_run where
   "wf_run L R oL oR (Leaf b) = True"
 | "wf_run L R oL oR (AskL i U1 U2) =
-     (i ∈ L ∧ wf_run L R oL oR (if oL i then U2 else U1))"
+     (i \<in> L \<and> wf_run L R oL oR (if oL i then U2 else U1))"
 | "wf_run L R oL oR (AskR j U1 U2) =
-     (j ∈ R ∧ wf_run L R oL oR (if oR j then U2 else U1))"
+     (j \<in> R \<and> wf_run L R oL oR (if oR j then U2 else U1))"
 
 fun tm_to_dtr' ::
-  "('C ⇒ int) ⇒ ('C ⇒ bool ⇒ 'C) ⇒ ('C ⇒ bool) ⇒ nat ⇒ 'C ⇒ (nat,nat) dtr"
+  "('C \<Rightarrow> int) \<Rightarrow> ('C \<Rightarrow> bool \<Rightarrow> 'C) \<Rightarrow> ('C \<Rightarrow> bool) \<Rightarrow> nat \<Rightarrow> 'C \<Rightarrow> (nat,nat) dtr"
 where
   "tm_to_dtr' head0 stepf final_acc 0 c = Leaf (final_acc c)"
 | "tm_to_dtr' head0 stepf final_acc (Suc t) c =
@@ -21,38 +21,38 @@ where
           (tm_to_dtr' head0 stepf final_acc t (stepf c True))"
 
 locale DTM_Run =
-  fixes steps   :: "'M ⇒ bool list ⇒ nat"          (* halting time on input x *)
-    and conf    :: "'M ⇒ bool list ⇒ nat ⇒ 'C"     (* configuration after t steps *)
-    and head0   :: "'C ⇒ int"                      (* position of input-tape head *)
-    and accepts :: "'M ⇒ bool list ⇒ bool"         (* acceptance predicate *)
+  fixes steps   :: "'M \<Rightarrow> bool list \<Rightarrow> nat"          (* halting time on input x *)
+    and conf    :: "'M \<Rightarrow> bool list \<Rightarrow> nat \<Rightarrow> 'C"     (* configuration after t steps *)
+    and head0   :: "'C \<Rightarrow> int"                      (* position of input-tape head *)
+    and accepts :: "'M \<Rightarrow> bool list \<Rightarrow> bool"         (* acceptance predicate *)
 begin
 
-definition read0 :: "'M ⇒ bool list ⇒ nat set" where
-  "read0 M x = (λt. nat (head0 (conf M x t))) ` {..< steps M x}"
+definition read0 :: "'M \<Rightarrow> bool list \<Rightarrow> nat set" where
+  "read0 M x = (\<lambda>t. nat (head0 (conf M x t))) ` {..< steps M x}"
 
 lemma finite_read0[simp]: "finite (read0 M x)"
   unfolding read0_def by (intro finite_imageI) simp
 
 lemma card_read0_le_steps:
-  "card (read0 M x) ≤ steps M x"
+  "card (read0 M x) \<le> steps M x"
   unfolding read0_def by (metis card_image_le card_lessThan finite_lessThan)
 
 end
 
-section ‹Contiguous overwrite (splice)›
+section \<open>Contiguous overwrite (splice)\<close>
 
-definition splice :: "nat ⇒ nat ⇒ bool list ⇒ bool list ⇒ bool list" where
+definition splice :: "nat \<Rightarrow> nat \<Rightarrow> bool list \<Rightarrow> bool list \<Rightarrow> bool list" where
   "splice a w xs bs = take a xs @ bs @ drop (a + w) xs"
 
 lemma splice_nth_inside:
   assumes LEN: "length bs = w"
-      and BND: "a + w ≤ length xs"
-      and IN1: "a ≤ i"
+      and BND: "a + w \<le> length xs"
+      and IN1: "a \<le> i"
       and IN2: "i < a + w"
   shows "splice a w xs bs ! i = bs ! (i - a)"
 proof -
   have ia_lt: "i - a < w" using IN1 IN2 by arith
-  have a_le_len: "a ≤ length xs" using BND by linarith
+  have a_le_len: "a \<le> length xs" using BND by linarith
   have "splice a w xs bs ! i = (take a xs @ bs @ drop (a + w) xs) ! i"
     by (simp add: splice_def)
   also have "... = (bs @ drop (a + w) xs) ! (i - a)"
@@ -63,20 +63,20 @@ proof -
 qed
 
 lemma splice_nth_left:
-  assumes BND: "a ≤ length xs"
+  assumes BND: "a \<le> length xs"
       and L:   "i < a"
   shows "splice a w xs bs ! i = xs ! i"
   using assms by (simp add: splice_def nth_append)
 
 lemma splice_nth_right:
   assumes LEN: "length bs = w"
-      and BND: "a + w ≤ length xs"
-      and R:   "a + w ≤ i"
+      and BND: "a + w \<le> length xs"
+      and R:   "a + w \<le> i"
   shows "splice a w xs bs ! i = xs ! i"
 proof -
-  have a_le_len: "a ≤ length xs" using BND by linarith
-  have i_ge_a:   "a ≤ i"         using R   by linarith
-  have i_minus_ge_w: "i - a ≥ w" using R   by arith
+  have a_le_len: "a \<le> length xs" using BND by linarith
+  have i_ge_a:   "a \<le> i"         using R   by linarith
+  have i_minus_ge_w: "i - a \<ge> w" using R   by arith
   have "splice a w xs bs ! i = (take a xs @ bs @ drop (a + w) xs) ! i"
     by (simp add: splice_def)
   also have "... = (bs @ drop (a + w) xs) ! (i - a)"
@@ -91,50 +91,50 @@ proof -
 qed
 
 lemma splice_outside_left:
-  assumes "i < a" "a ≤ length xs"
+  assumes "i < a" "a \<le> length xs"
   shows   "splice a w xs ys ! i = xs ! i"
   using assms by (simp add: splice_nth_left)
 
 lemma splice_outside_right:
-  assumes "a + w ≤ i" "length ys = w" "a + w ≤ length xs"
+  assumes "a + w \<le> i" "length ys = w" "a + w \<le> length xs"
   shows   "splice a w xs ys ! i = xs ! i"
   using assms by (simp add: splice_nth_right)
 
-section ‹DTM semantics sufficient for unread-agreement›
+section \<open>DTM semantics sufficient for unread-agreement\<close>
 
 locale DTM_Run_Sem =
-  fixes steps     :: "'M ⇒ bool list ⇒ nat"
-    and conf      :: "'M ⇒ bool list ⇒ nat ⇒ 'C"
-    and head0     :: "'C ⇒ int"
-    and accepts   :: "'M ⇒ bool list ⇒ bool"
+  fixes steps     :: "'M \<Rightarrow> bool list \<Rightarrow> nat"
+    and conf      :: "'M \<Rightarrow> bool list \<Rightarrow> nat \<Rightarrow> 'C"
+    and head0     :: "'C \<Rightarrow> int"
+    and accepts   :: "'M \<Rightarrow> bool list \<Rightarrow> bool"
     and M         :: 'M
-    and stepf     :: "'C ⇒ bool ⇒ 'C"
-    and final_acc :: "'C ⇒ bool"
+    and stepf     :: "'C \<Rightarrow> bool \<Rightarrow> 'C"
+    and final_acc :: "'C \<Rightarrow> bool"
   assumes step_sem:
-    "⋀x t. conf M x (Suc t) = stepf (conf M x t) (x ! nat (head0 (conf M x t)))"
+    "\<And>x t. conf M x (Suc t) = stepf (conf M x t) (x ! nat (head0 (conf M x t)))"
   assumes steps_stable_raw:
-    "⋀x y. (⋀i. i ∈ ((λt. nat (head0 (conf M x t))) ` {..< steps M x}) ⟹ x ! i = y ! i)
-           ⟹ steps M x = steps M y"
+    "\<And>x y. (\<And>i. i \<in> ((\<lambda>t. nat (head0 (conf M x t))) ` {..< steps M x}) \<Longrightarrow> x ! i = y ! i)
+           \<Longrightarrow> steps M x = steps M y"
   assumes accepts_sem:
-    "⋀x. accepts M x = final_acc (conf M x (steps M x))"
-  assumes conf0_same: "⋀x y. conf M x 0 = conf M y 0"
+    "\<And>x. accepts M x = final_acc (conf M x (steps M x))"
+  assumes conf0_same: "\<And>x y. conf M x 0 = conf M y 0"
 begin
 
-primrec drive :: "nat ⇒ 'C ⇒ (nat ⇒ bool) ⇒ 'C" where
+primrec drive :: "nat \<Rightarrow> 'C \<Rightarrow> (nat \<Rightarrow> bool) \<Rightarrow> 'C" where
   "drive 0 c inp = c"
 | "drive (Suc t) c inp =
      (let i = nat (head0 c); b = inp i in drive t (stepf c b) inp)"
 
 lemma drive_conf_gen:
-  "drive t (conf M x u) (λi. x ! i) = conf M x (u + t)"
+  "drive t (conf M x u) (\<lambda>i. x ! i) = conf M x (u + t)"
 proof (induction t arbitrary: u)
   case 0 show ?case by simp
 next
   case (Suc t)
-  have "drive (Suc t) (conf M x u) (λi. x ! i)
-        = drive t (stepf (conf M x u) (x ! nat (head0 (conf M x u)))) (λi. x ! i)"
+  have "drive (Suc t) (conf M x u) (\<lambda>i. x ! i)
+        = drive t (stepf (conf M x u) (x ! nat (head0 (conf M x u)))) (\<lambda>i. x ! i)"
     by simp
-  also have "... = drive t (conf M x (Suc u)) (λi. x ! i)"
+  also have "... = drive t (conf M x (Suc u)) (\<lambda>i. x ! i)"
     by (simp add: step_sem)
   also have "... = conf M x (Suc u + t)"
     by (simp add: Suc.IH)
@@ -142,7 +142,7 @@ next
 qed
 
 lemma drive_conf:
-  "drive t (conf M x 0) (λi. x ! i) = conf M x t"
+  "drive t (conf M x 0) (\<lambda>i. x ! i) = conf M x t"
   by (simp add: drive_conf_gen)
 
 (* Decision tree eval matches the driven TM evolution *)
@@ -153,30 +153,30 @@ lemma run_tm_to_dtr':
 
 (* Specialize to x and steps M x *)
 lemma tm_to_dtr_correct:
-  "run (λi. x ! i) (λi. x ! i)
+  "run (\<lambda>i. x ! i) (\<lambda>i. x ! i)
         (tm_to_dtr' head0 stepf final_acc (steps M x) (conf M x 0))
    = final_acc (conf M x (steps M x))"
   by (simp add: run_tm_to_dtr' drive_conf)
 
 corollary tm_to_dtr_accepts:
-  "run (λi. x ! i) (λi. x ! i)
+  "run (\<lambda>i. x ! i) (\<lambda>i. x ! i)
         (tm_to_dtr' head0 stepf final_acc (steps M x) (conf M x 0))
    = accepts M x"
   by (simp add: tm_to_dtr_correct accepts_sem)
 
 (* local read-set, if you need it later *)
-definition read0S :: "bool list ⇒ nat set" where
-  "read0S x = (λt. nat (head0 (conf M x t))) ` {..< steps M x}"
+definition read0S :: "bool list \<Rightarrow> nat set" where
+  "read0S x = (\<lambda>t. nat (head0 (conf M x t))) ` {..< steps M x}"
 
 (* handy: one-step shift for images over {..<t} to {..<Suc t} *)
 lemma image_shift_suc_subset:
-  fixes F :: "nat ⇒ 'a"
-  shows "(λu. F u) ` {..<t} ⊆ F ` {..<Suc t}"
+  fixes F :: "nat \<Rightarrow> 'a"
+  shows "(\<lambda>u. F u) ` {..<t} \<subseteq> F ` {..<Suc t}"
   by auto
 
 lemma seenL_tm_to_dtr_subset_read0_helper:
   "seenL_run oL oR (tm_to_dtr' head0 stepf final_acc t c)
-     ⊆ (λu. nat (head0 (drive u c oL))) ` {..< t}"
+     \<subseteq> (\<lambda>u. nat (head0 (drive u c oL))) ` {..< t}"
 proof (induction t arbitrary: c)
   case 0
   show ?case by simp
@@ -185,33 +185,33 @@ next
   let ?i = "nat (head0 c)"
 
   have root_in:
-    "?i ∈ (λu. nat (head0 (drive u c oL))) ` {..< Suc t}"
+    "?i \<in> (\<lambda>u. nat (head0 (drive u c oL))) ` {..< Suc t}"
     by (rule image_eqI[where x=0]) simp_all
 
   have IH_sub:
     "seenL_run oL oR
        (tm_to_dtr' head0 stepf final_acc t (stepf c (oL ?i)))
-     ⊆ (λu. nat (head0 (drive u (stepf c (oL ?i)) oL))) ` {..< t}"
+     \<subseteq> (\<lambda>u. nat (head0 (drive u (stepf c (oL ?i)) oL))) ` {..< t}"
     by (rule Suc.IH)
 
   have drive_suc:
-    "(λu. nat (head0 (drive u (stepf c (oL ?i)) oL)))
-     = (λu. nat (head0 (drive (Suc u) c oL)))"
+    "(\<lambda>u. nat (head0 (drive u (stepf c (oL ?i)) oL)))
+     = (\<lambda>u. nat (head0 (drive (Suc u) c oL)))"
     by (intro ext) simp
 
   have sub_into_parent:
-    "(λu. nat (head0 (drive (Suc u) c oL))) ` {..< t}
-     ⊆ (λu. nat (head0 (drive u c oL))) ` {..< Suc t}"
+    "(\<lambda>u. nat (head0 (drive (Suc u) c oL))) ` {..< t}
+     \<subseteq> (\<lambda>u. nat (head0 (drive u c oL))) ` {..< Suc t}"
   proof
     fix y
-    assume "y ∈ (λu. nat (head0 (drive (Suc u) c oL))) ` {..< t}"
+    assume "y \<in> (\<lambda>u. nat (head0 (drive (Suc u) c oL))) ` {..< t}"
     then obtain u where u_lt: "u < t"
       and y_def: "y = nat (head0 (drive (Suc u) c oL))" by auto
-    have "y = (λv. nat (head0 (drive v c oL))) (Suc u)"
+    have "y = (\<lambda>v. nat (head0 (drive v c oL))) (Suc u)"
       by (simp add: y_def)
-    moreover have "Suc u ∈ {..< Suc t}"
+    moreover have "Suc u \<in> {..< Suc t}"
       using u_lt by simp
-    ultimately show "y ∈ (λu. nat (head0 (drive u c oL))) ` {..< Suc t}"
+    ultimately show "y \<in> (\<lambda>u. nat (head0 (drive u c oL))) ` {..< Suc t}"
       by (rule image_eqI)
   qed
 
@@ -229,17 +229,17 @@ sublocale Base: DTM_Run steps conf head0 accepts .
 
 lemma seenL_tm_to_dtr_subset_read0:
   fixes x :: "bool list"
-  defines "T ≡ tm_to_dtr' head0 stepf final_acc (steps M x) (conf M x 0)"
-  shows "seenL_run (λi. x ! i) (λj. x ! j) T ⊆ Base.read0 M x"
+  defines "T \<equiv> tm_to_dtr' head0 stepf final_acc (steps M x) (conf M x 0)"
+  shows "seenL_run (\<lambda>i. x ! i) (\<lambda>j. x ! j) T \<subseteq> Base.read0 M x"
 proof -
   have A:
-    "seenL_run (λi. x ! i) (λj. x ! j)
+    "seenL_run (\<lambda>i. x ! i) (\<lambda>j. x ! j)
        (tm_to_dtr' head0 stepf final_acc (steps M x) (conf M x 0))
-     ⊆ (λu. nat (head0 (drive u (conf M x 0) (λi. x ! i)))) ` {..< steps M x}"
+     \<subseteq> (\<lambda>u. nat (head0 (drive u (conf M x 0) (\<lambda>i. x ! i)))) ` {..< steps M x}"
     by (rule seenL_tm_to_dtr_subset_read0_helper)
-  also have "… = (λu. nat (head0 (conf M x u))) ` {..< steps M x}"
+  also have "\<dots> = (\<lambda>u. nat (head0 (conf M x u))) ` {..< steps M x}"
     by (simp add: drive_conf)
-  also have "… = Base.read0 M x"
+  also have "\<dots> = Base.read0 M x"
     unfolding Base.read0_def by simp
   finally show ?thesis by (simp add: T_def)
 qed
@@ -247,7 +247,7 @@ qed
 (* 1) Helper proved by induction on t *)
 lemma seenR_tm_to_dtr_subset_read0_helper:
   "seenR_run oL oR (tm_to_dtr' head0 stepf final_acc t c)
-     ⊆ (λu. nat (head0 (drive u c oL))) ` {..< t}"
+     \<subseteq> (\<lambda>u. nat (head0 (drive u c oL))) ` {..< t}"
 proof (induction t arbitrary: c)
   case 0
   show ?case by simp
@@ -260,25 +260,25 @@ next
     by simp
   have IH_sub:
     "seenR_run oL oR (tm_to_dtr' head0 stepf final_acc t (stepf c (oL ?i)))
-       ⊆ (λu. nat (head0 (drive u (stepf c (oL ?i)) oL))) ` {..< t}"
+       \<subseteq> (\<lambda>u. nat (head0 (drive u (stepf c (oL ?i)) oL))) ` {..< t}"
     by (rule Suc.IH)
   have drive_suc:
-    "(λu. nat (head0 (drive u (stepf c (oL ?i)) oL)))
-     = (λu. nat (head0 (drive (Suc u) c oL)))"
+    "(\<lambda>u. nat (head0 (drive u (stepf c (oL ?i)) oL)))
+     = (\<lambda>u. nat (head0 (drive (Suc u) c oL)))"
     by (intro ext) simp
   have shift:
-    "(λu. nat (head0 (drive (Suc u) c oL))) ` {..< t}
-       ⊆ (λu. nat (head0 (drive u c oL))) ` {..< Suc t}"
+    "(\<lambda>u. nat (head0 (drive (Suc u) c oL))) ` {..< t}
+       \<subseteq> (\<lambda>u. nat (head0 (drive u c oL))) ` {..< Suc t}"
   proof
-    fix y assume "y ∈ (λu. nat (head0 (drive (Suc u) c oL))) ` {..< t}"
+    fix y assume "y \<in> (\<lambda>u. nat (head0 (drive (Suc u) c oL))) ` {..< t}"
     then obtain u where u:"u < t" and y:"y = nat (head0 (drive (Suc u) c oL))" by auto
-    have "Suc u ∈ {..< Suc t}" using u by simp
-    have mem: "Suc u ∈ {..< Suc t}" using u by simp
-    have eq:  "y = (λv. nat (head0 (drive v c oL))) (Suc u)" by (simp add: y)
-    have "(λv. nat (head0 (drive v c oL))) (Suc u)
-        ∈ (λv. nat (head0 (drive v c oL))) ` {..< Suc t}"
+    have "Suc u \<in> {..< Suc t}" using u by simp
+    have mem: "Suc u \<in> {..< Suc t}" using u by simp
+    have eq:  "y = (\<lambda>v. nat (head0 (drive v c oL))) (Suc u)" by (simp add: y)
+    have "(\<lambda>v. nat (head0 (drive v c oL))) (Suc u)
+        \<in> (\<lambda>v. nat (head0 (drive v c oL))) ` {..< Suc t}"
       using mem by (rule imageI)
-    thus "y ∈ (λv. nat (head0 (drive v c oL))) ` {..< Suc t}"
+    thus "y \<in> (\<lambda>v. nat (head0 (drive v c oL))) ` {..< Suc t}"
       by (simp add: eq)
   qed
   from split IH_sub drive_suc shift show ?case by auto
@@ -287,17 +287,17 @@ qed
 (* 2) Use the helper to get the version w.r.t. Base.read0 *)
 lemma seenR_tm_to_dtr_subset_read0:
   fixes x :: "bool list"
-  defines "T ≡ tm_to_dtr' head0 stepf final_acc (steps M x) (conf M x 0)"
-  shows "seenR_run (λi. x ! i) (λj. x ! j) T ⊆ Base.read0 M x"
+  defines "T \<equiv> tm_to_dtr' head0 stepf final_acc (steps M x) (conf M x 0)"
+  shows "seenR_run (\<lambda>i. x ! i) (\<lambda>j. x ! j) T \<subseteq> Base.read0 M x"
 proof -
   have
-    "seenR_run (λi. x ! i) (λj. x ! j)
+    "seenR_run (\<lambda>i. x ! i) (\<lambda>j. x ! j)
        (tm_to_dtr' head0 stepf final_acc (steps M x) (conf M x 0))
-     ⊆ (λu. nat (head0 (drive u (conf M x 0) (λi. x ! i)))) ` {..< steps M x}"
+     \<subseteq> (\<lambda>u. nat (head0 (drive u (conf M x 0) (\<lambda>i. x ! i)))) ` {..< steps M x}"
     by (rule seenR_tm_to_dtr_subset_read0_helper)
-  also have "… = (λu. nat (head0 (conf M x u))) ` {..< steps M x}"
+  also have "\<dots> = (\<lambda>u. nat (head0 (conf M x u))) ` {..< steps M x}"
     by (simp add: drive_conf)
-  also have "… = Base.read0 M x"
+  also have "\<dots> = Base.read0 M x"
     unfolding Base.read0_def by simp
   finally show ?thesis by (simp add: T_def)
 qed
@@ -307,16 +307,16 @@ lemma read0_bridge: "read0S x = Base.read0 M x"
   by (simp add: read0S_def Base.read0_def)
 
 lemma steps_stable:
-  assumes AG: "⋀i. i ∈ Base.read0 M x ⟹ x ! i = y ! i"
+  assumes AG: "\<And>i. i \<in> Base.read0 M x \<Longrightarrow> x ! i = y ! i"
   shows "steps M x = steps M y"
 proof (rule steps_stable_raw)
   fix i
-  assume iIn: "i ∈ (λt. nat (head0 (conf M x t))) ` {..< steps M x}"
+  assume iIn: "i \<in> (\<lambda>t. nat (head0 (conf M x t))) ` {..< steps M x}"
   (* 1) Turn it into membership in the local read-set *)
-  have iR0S: "i ∈ read0S x"
+  have iR0S: "i \<in> read0S x"
     using iIn by (simp add: read0S_def)
   (* 2) Bridge to the locale’s read-set *)
-  have iBase: "i ∈ Base.read0 M x"
+  have iBase: "i \<in> Base.read0 M x"
     using iR0S by (simp add: read0_bridge)
   (* 3) Apply the assumption *)
   show "x ! i = y ! i" by (rule AG[OF iBase])
@@ -325,47 +325,47 @@ qed
 (* helper: if t < steps, the index read at time t is in read0S *)
 lemma idx_in_read0S:
   assumes "t < steps M x"
-  shows "nat (head0 (conf M x t)) ∈ read0S x"
+  shows "nat (head0 (conf M x t)) \<in> read0S x"
   using assms
   unfolding read0S_def
   by (intro image_eqI[where x=t]) simp_all
 
 lemma unread_agreement:
-  assumes AG: "⋀i. i ∈ Base.read0 M x ⟹ x ! i = y ! i"
-  shows "accepts M x ⟷ accepts M y"
+  assumes AG: "\<And>i. i \<in> Base.read0 M x \<Longrightarrow> x ! i = y ! i"
+  shows "accepts M x \<longleftrightarrow> accepts M y"
 proof -
   (* same halting time *)
   have steps_eq: "steps M x = steps M y"
     by (rule steps_stable[OF AG])
 
   (* convert agreement to the local read-set once *)
-  have AGS: "⋀i. i ∈ read0S x ⟹ x ! i = y ! i"
+  have AGS: "\<And>i. i \<in> read0S x \<Longrightarrow> x ! i = y ! i"
   proof -
-    fix i assume "i ∈ read0S x"
-    hence "i ∈ Base.read0 M x" by (simp add: read0_bridge)
+    fix i assume "i \<in> read0S x"
+    hence "i \<in> Base.read0 M x" by (simp add: read0_bridge)
     thus "x ! i = y ! i" by (rule AG)
   qed
 
   (* configurations match up to the halting time *)
-  have conf_eq: "⋀t. t ≤ steps M x ⟹ conf M x t = conf M y t"
+  have conf_eq: "\<And>t. t \<le> steps M x \<Longrightarrow> conf M x t = conf M y t"
   proof-
     fix t :: nat
-    show "t ≤ steps M x ⟹ conf M x t = conf M y t"
+    show "t \<le> steps M x \<Longrightarrow> conf M x t = conf M y t"
     proof (induction t)
       case 0
       show ?case by (simp add: conf0_same) 
     next
       case (Suc t)
-  (* from Suc t ≤ steps … get the strict bound we actually need *)
+  (* from Suc t \<le> steps \<dots> get the strict bound we actually need *)
       have t_lt: "t < steps M x" using Suc.prems by simp
 
-  (* apply IH at t ≤ steps … *)
+  (* apply IH at t \<le> steps \<dots> *)
       have IH: "conf M x t = conf M y t" by (rule Suc.IH) (use Suc.prems in simp)
 
       let ?i = "nat (head0 (conf M x t))"
 
   (* the scanned index at time t is in the read-set *)
-      have i_mem: "?i ∈ read0S x"
+      have i_mem: "?i \<in> read0S x"
         unfolding read0S_def
         by (intro image_eqI[where x=t]) (use t_lt in simp_all)
 
@@ -398,14 +398,14 @@ proof -
   finally show ?thesis .
 qed
 
-abbreviation sp :: "nat ⇒ nat ⇒ bool list ⇒ bool list ⇒ bool list" where
-  "sp ≡ SubsetSum_DTM_Bridge.splice"
+abbreviation sp :: "nat \<Rightarrow> nat \<Rightarrow> bool list \<Rightarrow> bool list \<Rightarrow> bool list" where
+  "sp \<equiv> SubsetSum_DTM_Bridge.splice"
 
 end
 
-section ‹Catalog blocks and padded encoding›
+section \<open>Catalog blocks and padded encoding\<close>
 
-text ‹We serialize the sets of LHS/RHS values into non-overlapping bit-blocks.›
+text \<open>We serialize the sets of LHS/RHS values into non-overlapping bit-blocks.\<close>
 
 definition enumL where
   "enumL as s k = sorted_list_of_set (LHS (e_k as s k) (length as))"
@@ -427,77 +427,77 @@ lemma enumR_set[simp]:
   "set (enumR as s k) = RHS (e_k as s k) (length as)"
   by (simp add: enumR_def)
 
-text ‹Fixed block width; later you can make it logarithmic in the values.›
-definition W :: "int list ⇒ int ⇒ nat" where
+text \<open>Fixed block width; later you can make it logarithmic in the values.\<close>
+definition W :: "int list \<Rightarrow> int \<Rightarrow> nat" where
   "W as s = max 1 (length as)"
 
-definition offL :: "int list ⇒ int ⇒ nat ⇒ nat" where
+definition offL :: "int list \<Rightarrow> int \<Rightarrow> nat \<Rightarrow> nat" where
   "offL as s j = j * W as s"
 
-definition offR :: "int list ⇒ int ⇒ nat ⇒ nat ⇒ nat" where
+definition offR :: "int list \<Rightarrow> int \<Rightarrow> nat \<Rightarrow> nat \<Rightarrow> nat" where
   "offR as s k j = length (enumL as s k) * W as s + j * W as s"
 
-definition blockL :: "int list ⇒ int ⇒ nat ⇒ nat set" where
+definition blockL :: "int list \<Rightarrow> int \<Rightarrow> nat \<Rightarrow> nat set" where
   "blockL as s j = { offL as s j ..< offL as s j + W as s }"
 
-definition blockR :: "int list ⇒ int ⇒ nat ⇒ nat ⇒ nat set" where
+definition blockR :: "int list \<Rightarrow> int \<Rightarrow> nat \<Rightarrow> nat \<Rightarrow> nat set" where
   "blockR as s k j = { offR as s k j ..< offR as s k j + W as s }"
 
 definition blockL_abs ::
-  "(int list ⇒ int ⇒ bool list) ⇒ int list ⇒ int ⇒ nat ⇒ nat set" where
+  "(int list \<Rightarrow> int \<Rightarrow> bool list) \<Rightarrow> int list \<Rightarrow> int \<Rightarrow> nat \<Rightarrow> nat set" where
   "blockL_abs E as s j =
      { length (E as s) + offL as s j ..<
        length (E as s) + offL as s j + W as s }"
 
 definition blockR_abs ::
-  "(int list ⇒ int ⇒ bool list) ⇒ int list ⇒ int ⇒ nat ⇒ nat ⇒ nat set" where
+  "(int list \<Rightarrow> int \<Rightarrow> bool list) \<Rightarrow> int list \<Rightarrow> int \<Rightarrow> nat \<Rightarrow> nat \<Rightarrow> nat set" where
   "blockR_abs E as s k j =
      { length (E as s) + offR as s k j ..<
        length (E as s) + offR as s k j + W as s }"
 
 lemma blockL_abs_disjoint:
-  assumes "j ≠ j'"
-  shows   "blockL_abs E as s j ∩ blockL_abs E as s j' = {}"
+  assumes "j \<noteq> j'"
+  shows   "blockL_abs E as s j \<inter> blockL_abs E as s j' = {}"
 proof -
   let ?W = "W as s"
   let ?c = "length (E as s)"
-  have "j < j' ∨ j' < j" using assms by arith
+  have "j < j' \<or> j' < j" using assms by arith
   then show ?thesis
   proof
     assume lt: "j < j'"
-    have "(Suc j) * ?W ≤ j' * ?W"
+    have "(Suc j) * ?W \<le> j' * ?W"
       using lt by (intro mult_right_mono) simp_all
-    hence "?c + j * ?W + ?W ≤ ?c + j' * ?W" by simp
+    hence "?c + j * ?W + ?W \<le> ?c + j' * ?W" by simp
     thus ?thesis by (auto simp: blockL_abs_def offL_def)
   next
     assume lt: "j' < j"
-    have "(Suc j') * ?W ≤ j * ?W"
+    have "(Suc j') * ?W \<le> j * ?W"
       using lt by (intro mult_right_mono) simp_all
-    hence "?c + j' * ?W + ?W ≤ ?c + j * ?W" by simp
+    hence "?c + j' * ?W + ?W \<le> ?c + j * ?W" by simp
     thus ?thesis by (auto simp: blockL_abs_def offL_def)
   qed
 qed
 
 lemma blockR_abs_disjoint:
-  assumes "j ≠ j'"
-  shows   "blockR_abs E as s k j ∩ blockR_abs E as s k j' = {}"
+  assumes "j \<noteq> j'"
+  shows   "blockR_abs E as s k j \<inter> blockR_abs E as s k j' = {}"
 proof -
   let ?W = "W as s"
   let ?c = "length (E as s)"
-  have "j < j' ∨ j' < j" using assms by arith
+  have "j < j' \<or> j' < j" using assms by arith
   then show ?thesis
   proof
     assume lt: "j < j'"
-    have "(Suc j) * ?W ≤ j' * ?W"
+    have "(Suc j) * ?W \<le> j' * ?W"
       using lt by (intro mult_right_mono) simp_all
-    hence "?c + offR as s k j + ?W ≤ ?c + offR as s k j'"
+    hence "?c + offR as s k j + ?W \<le> ?c + offR as s k j'"
       by (simp add: offR_def add_mult_distrib2)
     thus ?thesis by (auto simp: blockR_abs_def)
   next
     assume lt: "j' < j"
-    have "(Suc j') * ?W ≤ j * ?W"
+    have "(Suc j') * ?W \<le> j * ?W"
       using lt by (intro mult_right_mono) simp_all
-    hence "?c + offR as s k j' + ?W ≤ ?c + offR as s k j"
+    hence "?c + offR as s k j' + ?W \<le> ?c + offR as s k j"
       by (simp add: offR_def add_mult_distrib2)
     thus ?thesis by (auto simp: blockR_abs_def)
   qed
@@ -505,17 +505,17 @@ qed
 
 lemma blockL_abs_blockR_abs_disjoint:
   assumes jL: "j < length (enumL as s k)"
-  shows   "blockL_abs E as s j ∩ blockR_abs E as s k j' = {}"
+  shows   "blockL_abs E as s j \<inter> blockR_abs E as s k j' = {}"
 proof -
   let ?W = "W as s"
   let ?c = "length (E as s)"
   have step:
-    "?c + offL as s j + ?W ≤ ?c + offR as s k j'"
+    "?c + offL as s j + ?W \<le> ?c + offR as s k j'"
   proof -
-    have "(Suc j) * ?W ≤ length (enumL as s k) * ?W"
+    have "(Suc j) * ?W \<le> length (enumL as s k) * ?W"
       using jL by (intro mult_right_mono) simp_all
-    hence "?c + (Suc j) * ?W ≤ ?c + length (enumL as s k) * ?W" by simp
-    also have "… ≤ ?c + (length (enumL as s k) * ?W + j' * ?W)" by simp
+    hence "?c + (Suc j) * ?W \<le> ?c + length (enumL as s k) * ?W" by simp
+    also have "\<dots> \<le> ?c + (length (enumL as s k) * ?W + j' * ?W)" by simp
     finally show ?thesis
       by (simp add: offL_def offR_def add_mult_distrib2)
   qed
@@ -526,58 +526,58 @@ qed
 (* same width, consecutive half-open blocks are disjoint when indices differ *)
 lemma blocks_disjoint_same_base:
   fixes W :: nat
-  assumes "W > 0" and "j ≠ j'"
-  shows "{j*W ..< j*W + W} ∩ {j'*W ..< j'*W + W} = {}"
+  assumes "W > 0" and "j \<noteq> j'"
+  shows "{j*W ..< j*W + W} \<inter> {j'*W ..< j'*W + W} = {}"
 proof -
-  have "j < j' ∨ j' < j" using assms(2) by arith
+  have "j < j' \<or> j' < j" using assms(2) by arith
   then show ?thesis
   proof
     assume lt: "j < j'"
-    have "(Suc j) * W ≤ j' * W"
+    have "(Suc j) * W \<le> j' * W"
       using lt assms(1) by (intro mult_right_mono) simp_all
-    hence "j*W + W ≤ j'*W" by simp
+    hence "j*W + W \<le> j'*W" by simp
     thus ?thesis by auto
   next
     assume lt: "j' < j"
-    have "(Suc j') * W ≤ j * W"
+    have "(Suc j') * W \<le> j * W"
       using lt assms(1) by (intro mult_right_mono) simp_all
-    hence "j'*W + W ≤ j*W" by simp
+    hence "j'*W + W \<le> j*W" by simp
     thus ?thesis by auto
   qed
 qed
 
 (* Disjointness results *)
 lemma blockL_disjoint:
-  assumes "j ≠ j'"
-  shows   "blockL as s j ∩ blockL as s j' = {}"
+  assumes "j \<noteq> j'"
+  shows   "blockL as s j \<inter> blockL as s j' = {}"
 proof -
   have Wpos: "W as s > 0" by (simp add: W_def)
   have base:
     "{offL as s j ..< offL as s j + W as s}
-     ∩ {offL as s j' ..< offL as s j' + W as s} = {}"
+     \<inter> {offL as s j' ..< offL as s j' + W as s} = {}"
     using blocks_disjoint_same_base[of "W as s" j j'] Wpos assms
     by (simp add: offL_def)
   show ?thesis using blockL_def base by simp
 qed
 
 lemma blockR_disjoint:
-  assumes "j ≠ j'"
-  shows "blockR as s k j ∩ blockR as s k j' = {}"
+  assumes "j \<noteq> j'"
+  shows "blockR as s k j \<inter> blockR as s k j' = {}"
 proof -
-  have "j < j' ∨ j' < j" using assms by arith
+  have "j < j' \<or> j' < j" using assms by arith
   then show ?thesis
   proof
     assume lt: "j < j'"
-    have "(Suc j) * W as s ≤ j' * W as s"
+    have "(Suc j) * W as s \<le> j' * W as s"
       using lt by (intro mult_right_mono) simp_all
-    hence "offR as s k j + W as s ≤ offR as s k j'"
+    hence "offR as s k j + W as s \<le> offR as s k j'"
       by (simp add: offR_def algebra_simps)   (* j*W + W = (Suc j)*W *)
     thus ?thesis by (auto simp: blockR_def)
   next
     assume lt: "j' < j"
-    have "(Suc j') * W as s ≤ j * W as s"
+    have "(Suc j') * W as s \<le> j * W as s"
       using lt by (intro mult_right_mono) simp_all
-    hence "offR as s k j' + W as s ≤ offR as s k j"
+    hence "offR as s k j' + W as s \<le> offR as s k j"
       by (simp add: offR_def algebra_simps)
     thus ?thesis by (auto simp: blockR_def)
   qed
@@ -585,46 +585,46 @@ qed
 
 lemma blockL_blockR_disjoint:
   assumes jL: "j < length (enumL as s k)"
-  shows "blockL as s j ∩ blockR as s k j' = {}"
+  shows "blockL as s j \<inter> blockR as s k j' = {}"
 proof -
   let ?W = "W as s"
   let ?base = "length (enumL as s k) * ?W"
 
-  have Suc_le: "Suc j ≤ length (enumL as s k)" using jL by simp
-  have topL: "offL as s j + ?W ≤ ?base"
+  have Suc_le: "Suc j \<le> length (enumL as s k)" using jL by simp
+  have topL: "offL as s j + ?W \<le> ?base"
   proof -
     have "offL as s j + ?W = (j + 1) * ?W"
       by (simp add: offL_def add_mult_distrib2)
-    also have "... ≤ length (enumL as s k) * ?W"
+    also have "... \<le> length (enumL as s k) * ?W"
       using Suc_le by (intro mult_right_mono) simp_all
     finally show ?thesis .
   qed
 
-  have "blockL as s j ⊆ {..< ?base}"
+  have "blockL as s j \<subseteq> {..< ?base}"
   proof
-    fix x assume xL: "x ∈ blockL as s j"
+    fix x assume xL: "x \<in> blockL as s j"
     have x_lt: "x < offL as s j + W as s"
       using xL by (simp add: blockL_def)
     have "x < length (enumL as s k) * W as s"
       using x_lt topL by (rule less_le_trans)
-    thus "x ∈ {..< length (enumL as s k) * W as s}"
+    thus "x \<in> {..< length (enumL as s k) * W as s}"
   by simp
   qed
   moreover
-  have "blockR as s k j' ⊆ {?base ..< ?base + ?W + j' * ?W}"
+  have "blockR as s k j' \<subseteq> {?base ..< ?base + ?W + j' * ?W}"
     by (auto simp: blockR_def offR_def W_def)
   ultimately show ?thesis by fastforce
 qed
 
-section ‹Padding encoder›
+section \<open>Padding encoder\<close>
 
 locale SubsetSum_Padded_Enc =
-  fixes enc0      :: "int list ⇒ int ⇒ bool list"     (* baseline CL encoding *)
-    and to_bits   :: "nat ⇒ int ⇒ bool list"           (* fixed-width bits of an integer *)
-    and from_bits :: "bool list ⇒ int"
+  fixes enc0      :: "int list \<Rightarrow> int \<Rightarrow> bool list"     (* baseline CL encoding *)
+    and to_bits   :: "nat \<Rightarrow> int \<Rightarrow> bool list"           (* fixed-width bits of an integer *)
+    and from_bits :: "bool list \<Rightarrow> int"
   assumes bits_roundtrip:
-    "⋀as s k v. v ∈ set (enumL as s k) ∪ set (enumR as s k) ⟹
-       length (to_bits (W as s) v) = W as s ∧ from_bits (to_bits (W as s) v) = v"
+    "\<And>as s k v. v \<in> set (enumL as s k) \<union> set (enumR as s k) \<Longrightarrow>
+       length (to_bits (W as s) v) = W as s \<and> from_bits (to_bits (W as s) v) = v"
 begin
 
 definition padL where
@@ -637,48 +637,48 @@ definition enc where
   "enc as s k = enc0 as s @ padL as s k @ padR as s k"
 
 (* Sum of a constant over any list *)
-lemma sum_const_all_nat: "(∑ _← L. (c::nat)) = length L * c" for L c
+lemma sum_const_all_nat: "(\<Sum> _\<leftarrow> L. (c::nat)) = length L * c" for L c
   by (induction L) simp_all
 
 (* helper: length rule on elements of enumL / enumR *)
 lemma to_bits_len_on_enumL:
-  assumes vL: "v ∈ set (enumL as s k)"
+  assumes vL: "v \<in> set (enumL as s k)"
   shows   "length (to_bits (W as s) v) = W as s"
 proof -
-  have inU: "v ∈ set (enumL as s k) ∪ set (enumR as s k)"
+  have inU: "v \<in> set (enumL as s k) \<union> set (enumR as s k)"
     using vL by auto   (* or: by (rule UnI1) *)
   from bits_roundtrip[OF inU] show ?thesis by simp
 qed
 
 lemma to_bits_len_on_enumR:
-  assumes vR: "v ∈ set (enumR as s k)"
+  assumes vR: "v \<in> set (enumR as s k)"
   shows   "length (to_bits (W as s) v) = W as s"
 proof -
-  have inU: "v ∈ set (enumL as s k) ∪ set (enumR as s k)"
+  have inU: "v \<in> set (enumL as s k) \<union> set (enumR as s k)"
     using vR by auto   (* or: by (rule UnI2) *)
   from bits_roundtrip[OF inU] show ?thesis by simp
 qed
 
 (* pointwise constant-length maps over the enumerations *)
 lemma map_len_to_bits_constL:
-  "map (λv. length (to_bits (W as s) v)) (enumL as s k)
-   = map (λ_. W as s) (enumL as s k)"
+  "map (\<lambda>v. length (to_bits (W as s) v)) (enumL as s k)
+   = map (\<lambda>_. W as s) (enumL as s k)"
   by (rule map_cong[OF refl]) (simp add: to_bits_len_on_enumL)
 
 lemma map_len_to_bits_constR:
-  "map (λv. length (to_bits (W as s) v)) (enumR as s k)
-   = map (λ_. W as s) (enumR as s k)"
+  "map (\<lambda>v. length (to_bits (W as s) v)) (enumR as s k)
+   = map (\<lambda>_. W as s) (enumR as s k)"
   by (rule map_cong[OF refl]) (simp add: to_bits_len_on_enumR)
 
 lemma length_padL:
   "length (padL as s k) = length (enumL as s k) * W as s"
 proof -
   have "length (padL as s k)
-        = sum_list (map (length ∘ to_bits (W as s)) (enumL as s k))"
+        = sum_list (map (length \<circ> to_bits (W as s)) (enumL as s k))"
     by (simp add: padL_def length_concat)
-  also have "... = sum_list (map (λv. length (to_bits (W as s) v)) (enumL as s k))"
+  also have "... = sum_list (map (\<lambda>v. length (to_bits (W as s) v)) (enumL as s k))"
     by (simp add: comp_def)
-  also have "... = sum_list (map (λ_. W as s) (enumL as s k))"
+  also have "... = sum_list (map (\<lambda>_. W as s) (enumL as s k))"
     by (simp add: map_len_to_bits_constL)
   also have "... = length (enumL as s k) * W as s"
     by (rule sum_const_all_nat)
@@ -689,11 +689,11 @@ lemma length_padR:
   "length (padR as s k) = length (enumR as s k) * W as s"
 proof -
   have "length (padR as s k)
-        = sum_list (map (length ∘ to_bits (W as s)) (enumR as s k))"
+        = sum_list (map (length \<circ> to_bits (W as s)) (enumR as s k))"
     by (simp add: padR_def length_concat)
-  also have "... = sum_list (map (λv. length (to_bits (W as s) v)) (enumR as s k))"
+  also have "... = sum_list (map (\<lambda>v. length (to_bits (W as s) v)) (enumR as s k))"
     by (simp add: comp_def)
-  also have "... = sum_list (map (λ_. W as s) (enumR as s k))"
+  also have "... = sum_list (map (\<lambda>_. W as s) (enumR as s k))"
     by (simp add: map_len_to_bits_constR)
   also have "... = length (enumR as s k) * W as s"
     by (rule sum_const_all_nat)
@@ -718,69 +718,69 @@ qed
 
 end
 
-section ‹Coverage via unread-agreement›
+section \<open>Coverage via unread-agreement\<close>
 
 locale Coverage_TM =
   DTM_Run_Sem steps conf head0 accepts M stepf final_acc +
   SubsetSum_Padded_Enc enc0 to_bits from_bits
-  for steps :: "'M ⇒ bool list ⇒ nat"
-  and conf  :: "'M ⇒ bool list ⇒ nat ⇒ 'C"
-  and head0 :: "'C ⇒ int"
-  and accepts :: "'M ⇒ bool list ⇒ bool"
+  for steps :: "'M \<Rightarrow> bool list \<Rightarrow> nat"
+  and conf  :: "'M \<Rightarrow> bool list \<Rightarrow> nat \<Rightarrow> 'C"
+  and head0 :: "'C \<Rightarrow> int"
+  and accepts :: "'M \<Rightarrow> bool list \<Rightarrow> bool"
   and M :: 'M
-  and stepf :: "'C ⇒ bool ⇒ 'C"
-  and final_acc :: "'C ⇒ bool"
-  and enc0  :: "int list ⇒ int ⇒ bool list"
-  and to_bits :: "nat ⇒ int ⇒ bool list"
-  and from_bits :: "bool list ⇒ int"
+  and stepf :: "'C \<Rightarrow> bool \<Rightarrow> 'C"
+  and final_acc :: "'C \<Rightarrow> bool"
+  and enc0  :: "int list \<Rightarrow> int \<Rightarrow> bool list"
+  and to_bits :: "nat \<Rightarrow> int \<Rightarrow> bool list"
+  and from_bits :: "bool list \<Rightarrow> int"
   +
 fixes kk :: nat
   (* NEW: define the locale-internal projections and predicate upfront *)
-  fixes Lval_at :: "int list ⇒ int ⇒ (nat ⇒ bool) ⇒ nat ⇒ int"
+  fixes Lval_at :: "int list \<Rightarrow> int \<Rightarrow> (nat \<Rightarrow> bool) \<Rightarrow> nat \<Rightarrow> int"
   defines Lval_at_def:
-    "Lval_at as s oL j ≡
+    "Lval_at as s oL j \<equiv>
        from_bits (map oL
          [length (enc0 as s) + offL as s j
           ..< length (enc0 as s) + offL as s j + W as s])"
 
-  fixes Rval_at :: "int list ⇒ int ⇒ (nat ⇒ bool) ⇒ nat ⇒ int"
+  fixes Rval_at :: "int list \<Rightarrow> int \<Rightarrow> (nat \<Rightarrow> bool) \<Rightarrow> nat \<Rightarrow> int"
   defines Rval_at_def:
-    "Rval_at as s oR j ≡
+    "Rval_at as s oR j \<equiv>
        from_bits (map oR
          [length (enc0 as s) + offR as s kk j
           ..< length (enc0 as s) + offR as s kk j + W as s])"
 
-  fixes good :: "int list ⇒ int ⇒ (nat ⇒ bool) ⇒ (nat ⇒ bool) ⇒ bool"
+  fixes good :: "int list \<Rightarrow> int \<Rightarrow> (nat \<Rightarrow> bool) \<Rightarrow> (nat \<Rightarrow> bool) \<Rightarrow> bool"
   defines good_def:
-    "good as s oL oR ≡
-       (∃jL<length (enumL as s kk). ∃jR<length (enumR as s kk).
+    "good as s oL oR \<equiv>
+       (\<exists>jL<length (enumL as s kk). \<exists>jR<length (enumR as s kk).
           Lval_at as s oL jL = Rval_at as s oR jR)"
 
   (* existing obligations: unchanged *)
   assumes correctness:
-    "⋀as s. accepts M (enc as s kk) =
+    "\<And>as s. accepts M (enc as s kk) =
             good as s ((!) (enc as s kk)) ((!) (enc as s kk))"
   and read0_after_enc0:
     "Base.read0 M (enc as s kk)
-       ⊆ { length (enc0 as s)
+       \<subseteq> { length (enc0 as s)
           ..< length (enc0 as s) + length (padL as s kk) + length (padR as s kk) }"
 begin
 
-abbreviation x0 :: "int list ⇒ int ⇒ bool list" where
-  "x0 as s ≡ enc as s kk"
+abbreviation x0 :: "int list \<Rightarrow> int \<Rightarrow> bool list" where
+  "x0 as s \<equiv> enc as s kk"
 
-definition touches :: "bool list ⇒ nat set ⇒ bool" where
-  "touches x B ⟷ Base.read0 M x ∩ B ≠ {}"
+definition touches :: "bool list \<Rightarrow> nat set \<Rightarrow> bool" where
+  "touches x B \<longleftrightarrow> Base.read0 M x \<inter> B \<noteq> {}"
 
 lemma offL_window_in_enc:
   assumes jL: "j < length (enumL as s kk)"
-  shows "length (enc0 as s) + offL as s j + W as s ≤ length (enc as s kk)"
+  shows "length (enc0 as s) + offL as s j + W as s \<le> length (enc as s kk)"
 proof -
   have pad_bound:
-    "offL as s j + W as s ≤ length (padL as s kk) + length (padR as s kk)"
+    "offL as s j + W as s \<le> length (padL as s kk) + length (padR as s kk)"
   proof -
     have "(Suc j) * W as s
-            ≤ (length (enumL as s kk) + length (enumR as s kk)) * W as s"
+            \<le> (length (enumL as s kk) + length (enumR as s kk)) * W as s"
       using jL by (intro mult_right_mono) simp_all
     then show ?thesis
       by (simp add: offL_def length_padL length_padR add_mult_distrib2 algebra_simps)
@@ -788,21 +788,21 @@ proof -
 
   have "length (enc0 as s) + offL as s j + W as s
         = length (enc0 as s) + (offL as s j + W as s)" by simp
-  also have "… ≤ length (enc0 as s) + (length (padL as s kk) + length (padR as s kk))"
+  also have "\<dots> \<le> length (enc0 as s) + (length (padL as s kk) + length (padR as s kk))"
     using pad_bound by (rule add_left_mono)
-  also have "… = length (enc as s kk)"
+  also have "\<dots> = length (enc as s kk)"
     by (simp add: enc_def)
   finally show ?thesis .
 qed
 
 lemma offR_window_in_enc:
   assumes jR: "j < length (enumR as s kk)"
-  shows "length (enc0 as s) + offR as s kk j + W as s ≤ length (enc as s kk)"
+  shows "length (enc0 as s) + offR as s kk j + W as s \<le> length (enc as s kk)"
 proof -
-  have "(Suc j) * W as s ≤ length (enumR as s kk) * W as s"
+  have "(Suc j) * W as s \<le> length (enumR as s kk) * W as s"
     using jR by (intro mult_right_mono) simp_all
   hence offR_le:
-    "offR as s kk j + W as s ≤ length (padL as s kk) + length (padR as s kk)"
+    "offR as s kk j + W as s \<le> length (padL as s kk) + length (padR as s kk)"
     by (simp add: offR_def length_padL length_padR add_mult_distrib2 algebra_simps)
   then show ?thesis
     by (simp add: enc_def add_left_mono)
@@ -810,39 +810,39 @@ qed
 
 (* 1) The index sets we want fully covered *)
 definition Lset where
-  "Lset as s ≡ ⋃ j < length (enumL as s kk). blockL_abs enc0 as s j"
+  "Lset as s \<equiv> \<Union> j < length (enumL as s kk). blockL_abs enc0 as s j"
 
 definition Rset where
-  "Rset as s ≡ ⋃ j < length (enumR as s kk). blockR_abs enc0 as s kk j"
+  "Rset as s \<equiv> \<Union> j < length (enumR as s kk). blockR_abs enc0 as s kk j"
 
 (* 2) The decision tree extracted from the TM on input x = enc as s kk *)
 definition T where
-  "T as s ≡
+  "T as s \<equiv>
      tm_to_dtr' head0 stepf final_acc
        (steps M (enc as s kk))
        (conf M (enc as s kk) 0)"
 
 lemma in_padL_imp_in_some_blockL_abs:
   assumes i_in:
-    "i ∈ {length (enc0 as s) ..< length (enc0 as s) + length (padL as s kk)}"
-  shows "∃j<length (enumL as s kk). i ∈ blockL_abs enc0 as s j"
+    "i \<in> {length (enc0 as s) ..< length (enc0 as s) + length (padL as s kk)}"
+  shows "\<exists>j<length (enumL as s kk). i \<in> blockL_abs enc0 as s j"
 proof -
   let ?len0 = "length (enc0 as s)"
   let ?W    = "W as s"
   let ?E    = "enumL as s kk"
   let ?k    = "i - ?len0"
 
-  have i_ge: "?len0 ≤ i" and i_lt: "i < ?len0 + length (padL as s kk)"
+  have i_ge: "?len0 \<le> i" and i_lt: "i < ?len0 + length (padL as s kk)"
     using i_in by auto
   hence k_lt: "?k < length (padL as s kk)" by simp
 
-  (* From membership, the padL interval is non-empty → W > 0 *)
+  (* From membership, the padL interval is non-empty \<rightarrow> W > 0 *)
   have Wpos: "0 < ?W"
   proof (rule ccontr)
-    assume "¬ 0 < ?W" hence "?W = 0" by simp
+    assume "\<not> 0 < ?W" hence "?W = 0" by simp
     hence "length (padL as s kk) = 0" by (simp add: length_padL)
-    have "length (padL as s kk) = 0" by (simp add: ‹length (padL as s kk) = 0›)
-    then have "i ∈ {length (enc0 as s) ..< length (enc0 as s) + 0}" using i_in by simp
+    have "length (padL as s kk) = 0" by (simp add: \<open>length (padL as s kk) = 0\<close>)
+    then have "i \<in> {length (enc0 as s) ..< length (enc0 as s) + 0}" using i_in by simp
     thus False by simp
   qed
 
@@ -866,7 +866,7 @@ proof -
   moreover have
     "blockL_abs enc0 as s j = { ?len0 + j * ?W ..< ?len0 + j * ?W + ?W }"
     by (simp add: blockL_abs_def offL_def)
-  ultimately have "i ∈ blockL_abs enc0 as s j"
+  ultimately have "i \<in> blockL_abs enc0 as s j"
     using r_lt by auto
 
   thus ?thesis by (intro exI[of _ j]) (use j_lt in simp)
@@ -874,15 +874,15 @@ qed
 
 lemma in_padR_imp_in_some_blockR_abs:
   assumes iR:
-    "i ∈ { length (enc0 as s) + length (padL as s kk)
+    "i \<in> { length (enc0 as s) + length (padL as s kk)
          ..< length (enc0 as s) + length (padL as s kk) + length (padR as s kk) }"
-  shows "∃j<length (enumR as s kk). i ∈ blockR_abs enc0 as s kk j"
+  shows "\<exists>j<length (enumR as s kk). i \<in> blockR_abs enc0 as s kk j"
 proof -
   let ?base = "length (enc0 as s) + length (padL as s kk)"
   let ?W    = "W as s"
   let ?r    = "i - ?base"
 
-  from iR have base_le: "?base ≤ i"
+  from iR have base_le: "?base \<le> i"
     and r_lt: "?r < length (padR as s kk)"
     by auto
 
@@ -892,7 +892,7 @@ proof -
   (* show W>0; otherwise padR would be empty, contradicting r_lt *)
   have Wpos: "0 < ?W"
   proof (rule ccontr)
-    assume "¬ 0 < ?W"
+    assume "\<not> 0 < ?W"
     then have "?W = 0" by simp
     then have "length (padR as s kk) = 0" by (simp add: padR_len)
     with r_lt show False by simp
@@ -908,7 +908,7 @@ proof -
     using Wpos by (simp add: u_def)
 
 (* from iR you likely already have: *)
-  have base_le: "?base ≤ i" and r_lt: "i - ?base < length (padR as s kk)"
+  have base_le: "?base \<le> i" and r_lt: "i - ?base < length (padR as s kk)"
     using iR by auto
 
 (* You also proved 0 < ?W as Wpos earlier. Now the decomposition: *)
@@ -927,14 +927,14 @@ proof -
      = { ?base + j * ?W ..< ?base + j * ?W + ?W }"
     using blockR_abs_def offR_def by (simp add: add.assoc length_padL)
 
-have u_ge0: "0 ≤ u" by simp   (* nat is nonnegative *)
+have u_ge0: "0 \<le> u" by simp   (* nat is nonnegative *)
 
 have mem:
-  "length (enc0 as s) + length (padL as s kk) + j * W as s ≤ i ∧
+  "length (enc0 as s) + length (padL as s kk) + j * W as s \<le> i \<and>
    i < length (enc0 as s) + length (padL as s kk) + j * W as s + W as s"
   using i_decomp j_def u_def u_lt by force
 
-have "i ∈ blockR_abs enc0 as s kk j"
+have "i \<in> blockR_abs enc0 as s kk j"
   using mem
   by (simp add: BR_eq)
 
@@ -942,9 +942,9 @@ have "i ∈ blockR_abs enc0 as s kk j"
 qed
 
 lemma read0_subset_blocks_abs:
-  "Base.read0 M (enc as s kk) ⊆ Lset as s ∪ Rset as s"
+  "Base.read0 M (enc as s kk) \<subseteq> Lset as s \<union> Rset as s"
 proof
-  fix i assume iR: "i ∈ Base.read0 M (enc as s kk)"
+  fix i assume iR: "i \<in> Base.read0 M (enc as s kk)"
 
   have len_enc:
     "length (enc as s kk)
@@ -953,57 +953,57 @@ proof
 
   (* 1) First, land i in the big half-open interval after enc0 *)
   from read0_after_enc0 iR have i_band:
-    "i ∈ { length (enc0 as s)
+    "i \<in> { length (enc0 as s)
          ..< length (enc0 as s) + length (padL as s kk) + length (padR as s kk) }"
     by (rule subsetD)
 
   (* 2) Split i_band into the two inequalities we will feed to the L/R lemmas *)
-  have base_le:   "length (enc0 as s) ≤ i"
+  have base_le:   "length (enc0 as s) \<le> i"
     and  i_lt_enc: "i < length (enc0 as s) + length (padL as s kk) + length (padR as s kk)"
     using i_band by auto
 
   (* 3) Case split: i lies either in padL or in padR *)
   have disj:
-    "i < length (enc0 as s) + length (padL as s kk) ∨
-     length (enc0 as s) + length (padL as s kk) ≤ i" by linarith
+    "i < length (enc0 as s) + length (padL as s kk) \<or>
+     length (enc0 as s) + length (padL as s kk) \<le> i" by linarith
 
-  from disj show "i ∈ Lset as s ∪ Rset as s"
+  from disj show "i \<in> Lset as s \<union> Rset as s"
   proof
     (* ---- L-branch ---- *)
     assume i_lt_L: "i < length (enc0 as s) + length (padL as s kk)"
     have i_in_padL_set:
-      "i ∈ { length (enc0 as s) ..< length (enc0 as s) + length (padL as s kk) }"
+      "i \<in> { length (enc0 as s) ..< length (enc0 as s) + length (padL as s kk) }"
       using base_le i_lt_L by simp
     from in_padL_imp_in_some_blockL_abs[OF i_in_padL_set]
     obtain j where jL: "j < length (enumL as s kk)"
-               and iBL: "i ∈ blockL_abs enc0 as s j" by blast
-    have "i ∈ Lset as s"
+               and iBL: "i \<in> blockL_abs enc0 as s j" by blast
+    have "i \<in> Lset as s"
       unfolding Lset_def by (intro UN_I[of j]) (use jL iBL in auto)
     thus ?thesis by simp
 
   next
     (* ---- R-branch ---- *)
-    assume ge: "length (enc0 as s) + length (padL as s kk) ≤ i"
+    assume ge: "length (enc0 as s) + length (padL as s kk) \<le> i"
     have i_in_padR_set:
-      "i ∈ { length (enc0 as s) + length (padL as s kk)
+      "i \<in> { length (enc0 as s) + length (padL as s kk)
            ..< length (enc0 as s) + length (padL as s kk) + length (padR as s kk) }"
       using ge i_lt_enc by simp
     from in_padR_imp_in_some_blockR_abs[OF i_in_padR_set]
     obtain j where jR: "j < length (enumR as s kk)"
-               and iBR: "i ∈ blockR_abs enc0 as s kk j" by blast
-    have "i ∈ Rset as s"
+               and iBR: "i \<in> blockR_abs enc0 as s kk j" by blast
+    have "i \<in> Rset as s"
       unfolding Rset_def by (intro UN_I[of j]) (use jR iBR in auto)
     thus ?thesis by simp
   qed
 qed
 
 lemma wf_of_seen_run:
-  assumes "seenL_run oL oR U ⊆ L" "seenR_run oL oR U ⊆ R"
+  assumes "seenL_run oL oR U \<subseteq> L" "seenR_run oL oR U \<subseteq> R"
   shows   "wf_run L R oL oR U"
   using assms by (induction U) (auto split: if_splits)
 
 lemma wf_T_union_run:
-  "wf_run (Lset as s ∪ Rset as s) (Lset as s ∪ Rset as s)
+  "wf_run (Lset as s \<union> Rset as s) (Lset as s \<union> Rset as s)
           ((!) (enc as s kk)) ((!) (enc as s kk))
           (tm_to_dtr' head0 stepf final_acc (steps M (enc as s kk))
                        (conf M (enc as s kk) 0))"
@@ -1014,24 +1014,24 @@ proof -
   (* your SL0 / SR0 / subset derivations exactly as you already have: *)
   have SL1:
     "seenL_run ((!) ?x) ((!) ?x) ?T
-       ⊆ (λu. nat (head0 (drive u (conf M ?x 0) ((!) ?x)))) ` {..< steps M ?x}"
+       \<subseteq> (\<lambda>u. nat (head0 (drive u (conf M ?x 0) ((!) ?x)))) ` {..< steps M ?x}"
     by (rule seenL_tm_to_dtr_subset_read0_helper)
-  have SL0: "seenL_run ((!) ?x) ((!) ?x) ?T ⊆ Base.read0 M ?x"
+  have SL0: "seenL_run ((!) ?x) ((!) ?x) ?T \<subseteq> Base.read0 M ?x"
     using SL1 by (simp add: drive_conf Base.read0_def)
 
   have SR1:
     "seenR_run ((!) ?x) ((!) ?x) ?T
-       ⊆ (λu. nat (head0 (drive u (conf M ?x 0) ((!) ?x)))) ` {..< steps M ?x}"
+       \<subseteq> (\<lambda>u. nat (head0 (drive u (conf M ?x 0) ((!) ?x)))) ` {..< steps M ?x}"
     by (rule seenR_tm_to_dtr_subset_read0_helper)
-  have SR0: "seenR_run ((!) ?x) ((!) ?x) ?T ⊆ Base.read0 M ?x"
+  have SR0: "seenR_run ((!) ?x) ((!) ?x) ?T \<subseteq> Base.read0 M ?x"
     using SR1 by (simp add: drive_conf Base.read0_def)
 
-  have R0_sub: "Base.read0 M ?x ⊆ Lset as s ∪ Rset as s"
+  have R0_sub: "Base.read0 M ?x \<subseteq> Lset as s \<union> Rset as s"
     by (rule read0_subset_blocks_abs)
 
-  have SL: "seenL_run ((!) ?x) ((!) ?x) ?T ⊆ Lset as s ∪ Rset as s"
+  have SL: "seenL_run ((!) ?x) ((!) ?x) ?T \<subseteq> Lset as s \<union> Rset as s"
     using SL0 R0_sub by auto
-  have SR: "seenR_run ((!) ?x) ((!) ?x) ?T ⊆ Lset as s ∪ Rset as s"
+  have SR: "seenR_run ((!) ?x) ((!) ?x) ?T \<subseteq> Lset as s \<union> Rset as s"
     using SR0 R0_sub by auto
 
   show ?thesis by (rule wf_of_seen_run[OF SL SR])
@@ -1039,24 +1039,24 @@ qed
 
 (* 5) Correctness of the tree wrt the spec *)
 lemma correct_T:
-  "run (λi. (enc as s kk) ! i) (λj. (enc as s kk) ! j) (T as s)
-   = good as s (λi. (enc as s kk) ! i) (λj. (enc as s kk) ! j)"
+  "run (\<lambda>i. (enc as s kk) ! i) (\<lambda>j. (enc as s kk) ! j) (T as s)
+   = good as s (\<lambda>i. (enc as s kk) ! i) (\<lambda>j. (enc as s kk) ! j)"
 proof -
-  have "run (λi. (enc as s kk) ! i) (λj. (enc as s kk) ! j) (T as s)
+  have "run (\<lambda>i. (enc as s kk) ! i) (\<lambda>j. (enc as s kk) ! j) (T as s)
         = run ((!) (enc as s kk)) ((!) (enc as s kk))
              (tm_to_dtr' head0 stepf final_acc (steps M (enc as s kk))
                 (conf M (enc as s kk) 0))"
     by (simp add: T_def)
-  also have "… = accepts M (enc as s kk)"
+  also have "\<dots> = accepts M (enc as s kk)"
     by (simp add: tm_to_dtr_accepts)   (* from DTM_Run_Sem context *)
-  also have "… = good as s (λi. (enc as s kk) ! i) (λj. (enc as s kk) ! j)"
+  also have "\<dots> = good as s (\<lambda>i. (enc as s kk) ! i) (\<lambda>j. (enc as s kk) ! j)"
     by (simp add: correctness)
   finally show ?thesis .
 qed
 
 lemma nth_concat_map_fixed:
-  fixes xs :: "'a list" and f :: "'a ⇒ 'b list" and w :: nat
-  assumes LEN: "⋀x. x ∈ set xs ⟹ length (f x) = w"
+  fixes xs :: "'a list" and f :: "'a \<Rightarrow> 'b list" and w :: nat
+  assumes LEN: "\<And>x. x \<in> set xs \<Longrightarrow> length (f x) = w"
     and j: "j < length xs"
     and t: "t < w"
   shows "concat (map f xs) ! (j*w + t) = f (xs!j) ! t"
@@ -1065,9 +1065,9 @@ proof -
   have pref_len: "length (concat (map f (take j xs))) = j * w"
   proof -
     have "length (concat (map f (take j xs)))
-        = sum_list (map (length ∘ f) (take j xs))"
+        = sum_list (map (length \<circ> f) (take j xs))"
       by (simp add: length_concat)
-    also have "... = (∑_← take j xs. w)"
+    also have "... = (\<Sum>_\<leftarrow> take j xs. w)"
       by (smt (verit) LEN comp_apply in_set_takeD map_eq_conv)
     also have "... = length (take j xs) * w"
       by (simp add: sum_const_all_nat)
@@ -1109,7 +1109,7 @@ proof -
   have slice:
     "map ((!) (x0 as s)) [?a ..< ?a + ?w] = to_bits (W as s) (enumL as s kk ! j)"
   proof (rule nth_equalityI)
-    have v_inL: "enumL as s kk ! j ∈ set (enumL as s kk)"
+    have v_inL: "enumL as s kk ! j \<in> set (enumL as s kk)"
       using jL in_set_conv_nth by metis
     have len_tobits[simp]:
       "length (to_bits (W as s) (enumL as s kk ! j)) = W as s"
@@ -1132,7 +1132,7 @@ proof -
       proof -
         have jpart: "j * ?w + t < (Suc j) * ?w"
           using tw by (simp add: add_mult_distrib2)
-        have mono: "(Suc j) * ?w ≤ length (enumL as s kk) * ?w"
+        have mono: "(Suc j) * ?w \<le> length (enumL as s kk) * ?w"
           using jL by (intro mult_right_mono) simp_all
         from jpart mono show ?thesis
           by (simp add: offL_def length_padL less_le_trans)
@@ -1153,17 +1153,17 @@ proof -
       finally show ?thesis .
     qed
     have fixed_len_meta:
-      "⋀x'. x' ∈ set (enumL as s kk) ⟹ length (to_bits (W as s) x') = W as s"
+      "\<And>x'. x' \<in> set (enumL as s kk) \<Longrightarrow> length (to_bits (W as s) x') = W as s"
       by (simp add: to_bits_len_on_enumL)
     thus "map ((!) (x0 as s)) [?a ..< ?a + ?w] ! t
           = to_bits (W as s) (enumL as s kk ! j) ! t"
       using nth_map idx
-      by (smt (verit) ‹t < length (map ((!) (x0 as s)) 
+      by (smt (verit) \<open>t < length (map ((!) (x0 as s)) 
         [length (enc0 as s) + offL as s j..< 
-        length (enc0 as s) + offL as s j + W as s])› jL 
+        length (enc0 as s) + offL as s j + W as s])\<close> jL 
         length_map nth_concat_map_fixed step_enc_pad tw)
   qed
-  have v_in: "enumL as s kk ! j ∈ set (enumL as s kk)"
+  have v_in: "enumL as s kk ! j \<in> set (enumL as s kk)"
     using jL in_set_conv_nth by metis
   have round: "from_bits (to_bits (W as s) (enumL as s kk ! j)) = enumL as s kk ! j"
     using SubsetSum_Padded_Enc.bits_roundtrip SubsetSum_Padded_Enc_axioms v_in 
@@ -1175,7 +1175,7 @@ qed
 lemma Rval_at_on_enc_block:
   fixes j :: nat
   assumes jR: "j < length (enumR as s kk)"
-  shows "Rval_at as s (λi. (enc as s kk) ! i) j = enumR as s kk ! j"
+  shows "Rval_at as s (\<lambda>i. (enc as s kk) ! i) j = enumR as s kk ! j"
 proof -
   let ?a = "length (enc0 as s) + offR as s kk j"
   let ?w = "W as s"
@@ -1206,7 +1206,7 @@ proof -
 
     (* fixed-width chunks inside padR *)
     have fixed_len_meta:
-      "⋀x. x ∈ set (enumR as s kk) ⟹ length (to_bits (W as s) x) = ?w"
+      "\<And>x. x \<in> set (enumR as s kk) \<Longrightarrow> length (to_bits (W as s) x) = ?w"
       by (simp add: to_bits_len_on_enumR)
 
     have "map ((!) (x0 as s)) [?a ..< ?a + ?w] ! t
@@ -1225,11 +1225,11 @@ proof -
         = from_bits (to_bits (W as s) (enumR as s kk ! j))"
     by (simp add: Rval_at_def map_slice_R)
 
-  have v_inR: "enumR as s kk ! j ∈ set (enumR as s kk)"
+  have v_inR: "enumR as s kk ! j \<in> set (enumR as s kk)"
     using jR in_set_conv_nth by metis
 
   have v_inU:
-    "enumR as s kk ! j ∈ set (enumL as s kk) ∪ set (enumR as s kk)"
+    "enumR as s kk ! j \<in> set (enumL as s kk) \<union> set (enumR as s kk)"
     using v_inR by (rule UnI2)
 
   have "from_bits (to_bits (W as s) (enumR as s kk ! j))
@@ -1245,19 +1245,19 @@ proof -
 qed
 
 lemma R_catalog_for_enc:
-  "set (map (Rval_at as s (λi. (enc as s kk) ! i))
+  "set (map (Rval_at as s (\<lambda>i. (enc as s kk) ! i))
              [0..<length (enumR as s kk)])
    = set (enumR as s kk)"
 proof -
   let ?n = "length (enumR as s kk)"
   have map_eq:
     "map (Rval_at as s ((!) (x0 as s))) [0..<?n]
-     = map (λj. enumR as s kk ! j) [0..<?n]"
+     = map (\<lambda>j. enumR as s kk ! j) [0..<?n]"
     by (rule map_cong[OF _])
        (simp_all add: Rval_at_on_enc_block)
 
   have set_map_nth:
-    "set (map (λj. enumR as s kk ! j) [0..<?n]) = set (enumR as s kk)"
+    "set (map (\<lambda>j. enumR as s kk ! j) [0..<?n]) = set (enumR as s kk)"
     using set_conv_nth by (simp add: map_nth)
 
   show ?thesis
@@ -1267,20 +1267,20 @@ qed
 lemma flipL_pointwise_enc:
   fixes j :: nat
   assumes jL:  "j < length (enumL as s kk)"
-      and L2:  "2 ≤ length (enumL as s kk)"
-      and hit:  "∃v∈set (enumL as s kk). v ∈ set (enumR as s kk)"
-      and miss: "∃v∈set (enumL as s kk). v ∉ set (enumR as s kk)"
+      and L2:  "2 \<le> length (enumL as s kk)"
+      and hit:  "\<exists>v\<in>set (enumL as s kk). v \<in> set (enumR as s kk)"
+      and miss: "\<exists>v\<in>set (enumL as s kk). v \<notin> set (enumR as s kk)"
       and baseline_only_j:
-        "good as s ((!) (x0 as s)) ((!) (x0 as s)) ⟶
-         (∀j'<length (enumL as s kk). j' ≠ j ⟶
-            Lval_at as s ((!) (x0 as s)) j' ∉ set (enumR as s kk))"
-  shows "∃oL'. (∀i. i ∉ blockL_abs enc0 as s j ⟶ oL' i = (x0 as s) ! i)
-              ∧ good as s oL' ((!) (x0 as s))
-                ≠ good as s ((!) (x0 as s)) ((!) (x0 as s))"
+        "good as s ((!) (x0 as s)) ((!) (x0 as s)) \<longrightarrow>
+         (\<forall>j'<length (enumL as s kk). j' \<noteq> j \<longrightarrow>
+            Lval_at as s ((!) (x0 as s)) j' \<notin> set (enumR as s kk))"
+  shows "\<exists>oL'. (\<forall>i. i \<notin> blockL_abs enc0 as s j \<longrightarrow> oL' i = (x0 as s) ! i)
+              \<and> good as s oL' ((!) (x0 as s))
+                \<noteq> good as s ((!) (x0 as s)) ((!) (x0 as s))"
 proof -
-  obtain v_in where v_inL: "v_in ∈ set (enumL as s kk)" and v_inR: "v_in ∈ set (enumR as s kk)"
+  obtain v_in where v_inL: "v_in \<in> set (enumL as s kk)" and v_inR: "v_in \<in> set (enumR as s kk)"
     using hit by blast
-  obtain v_out where v_outL: "v_out ∈ set (enumL as s kk)" and v_outNR: "v_out ∉ set (enumR as s kk)"
+  obtain v_out where v_outL: "v_out \<in> set (enumL as s kk)" and v_outNR: "v_out \<notin> set (enumR as s kk)"
     using miss by blast
 
   let ?a = "length (enc0 as s) + offL as s j"
@@ -1291,8 +1291,8 @@ proof -
   obtain bv_out where bv_out_len: "length bv_out = ?w" and bv_out_val: "from_bits bv_out = v_out"
     using v_outL bits_roundtrip by blast
 
-  define oL_in  where "oL_in  i = (if i ∈ blockL_abs enc0 as s j then bv_in  ! (i - ?a) else (x0 as s) ! i)" for i
-  define oL_out where "oL_out i = (if i ∈ blockL_abs enc0 as s j then bv_out ! (i - ?a) else (x0 as s) ! i)" for i
+  define oL_in  where "oL_in  i = (if i \<in> blockL_abs enc0 as s j then bv_in  ! (i - ?a) else (x0 as s) ! i)" for i
+  define oL_out where "oL_out i = (if i \<in> blockL_abs enc0 as s j then bv_out ! (i - ?a) else (x0 as s) ! i)" for i
 
   have blk_eq: "blockL_abs enc0 as s j = {?a ..< ?a + ?w}"
     by (simp add: blockL_abs_def offL_def)
@@ -1307,7 +1307,7 @@ proof -
       fix t assume "t < length (map oL_in [?a ..< ?a + ?w])"
       hence tw: "t < ?w" by simp
       have idx: "[?a ..< ?a + ?w] ! t = ?a + t" using tw by simp
-      have inblk: "?a + t ∈ blockL_abs enc0 as s j" using tw by (simp add: blk_eq)
+      have inblk: "?a + t \<in> blockL_abs enc0 as s j" using tw by (simp add: blk_eq)
       show "map oL_in [?a ..< ?a + ?w] ! t = bv_in ! t"
         using nth_map idx oL_in_def inblk by (simp add: tw)
     qed
@@ -1323,18 +1323,18 @@ proof -
       fix t assume "t < length (map oL_out [?a ..< ?a + ?w])"
       hence tw: "t < ?w" by simp
       have idx: "[?a ..< ?a + ?w] ! t = ?a + t" using tw by simp
-      have inblk: "?a + t ∈ blockL_abs enc0 as s j" using tw by (simp add: blk_eq)
+      have inblk: "?a + t \<in> blockL_abs enc0 as s j" using tw by (simp add: blk_eq)
       show "map oL_out [?a ..< ?a + ?w] ! t = bv_out ! t"
         using nth_map idx oL_out_def inblk by (simp add: tw)
     qed
     show ?thesis by (simp add: Lval_at_def slice bv_out_val)
   qed
 
-  (* unchanged slices for j' ≠ j *)
+  (* unchanged slices for j' \<noteq> j *)
   have same_block:
-    "⋀j'. j' ≠ j ⟹ Lval_at as s oL_out j' = Lval_at as s ((!) (x0 as s)) j'"
+    "\<And>j'. j' \<noteq> j \<Longrightarrow> Lval_at as s oL_out j' = Lval_at as s ((!) (x0 as s)) j'"
   proof -
-    fix j' assume ne: "j' ≠ j"
+    fix j' assume ne: "j' \<noteq> j"
     let ?a' = "length (enc0 as s) + offL as s j'"
     let ?w' = "W as s"
     have blk': "blockL_abs enc0 as s j' = {?a' ..< ?a' + ?w'}"
@@ -1348,8 +1348,8 @@ proof -
       fix t assume "t < length (map oL_out [?a' ..< ?a' + ?w'])"
       hence tw: "t < ?w'" by simp
       have idx: "[?a' ..< ?a' + ?w'] ! t = ?a' + t" using tw by simp
-      have in_j': "?a' + t ∈ blockL_abs enc0 as s j'" using tw by (simp add: blk')
-      have not_in_j: "?a' + t ∉ blockL_abs enc0 as s j"
+      have in_j': "?a' + t \<in> blockL_abs enc0 as s j'" using tw by (simp add: blk')
+      have not_in_j: "?a' + t \<notin> blockL_abs enc0 as s j"
         using blockL_abs_disjoint[OF ne] in_j' by auto
       have out_eq: "oL_out (?a' + t) = (x0 as s) ! (?a' + t)"
         by (simp add: oL_out_def not_in_j)
@@ -1369,20 +1369,20 @@ proof -
 
   have Good_char:
     "good as s oL ((!) (x0 as s))
-     ⟷ (∃jL<length (enumL as s kk). Lval_at as s oL jL ∈ set (enumR as s kk))"
+     \<longleftrightarrow> (\<exists>jL<length (enumL as s kk). Lval_at as s oL jL \<in> set (enumR as s kk))"
     for oL
   proof
     assume "good as s oL ((!) (x0 as s))"
     then obtain jL jR where jL: "jL < length (enumL as s kk)" and jR: "jR < length (enumR as s kk)"
       and eq: "Lval_at as s oL jL = Rval_at as s ((!) (x0 as s)) jR"
       by (auto simp: good_def)
-    hence "Lval_at as s oL jL ∈ set (enumR as s kk)"
+    hence "Lval_at as s oL jL \<in> set (enumR as s kk)"
       using R_catalog jR by (auto simp: in_set_conv_nth)
-    thus "∃jL<length (enumL as s kk). Lval_at as s oL jL ∈ set (enumR as s kk)" using jL by blast
+    thus "\<exists>jL<length (enumL as s kk). Lval_at as s oL jL \<in> set (enumR as s kk)" using jL by blast
   next
-    assume "∃jL<length (enumL as s kk). Lval_at as s oL jL ∈ set (enumR as s kk)"
+    assume "\<exists>jL<length (enumL as s kk). Lval_at as s oL jL \<in> set (enumR as s kk)"
     then obtain jL where jL: "jL < length (enumL as s kk)"
-      and mem: "Lval_at as s oL jL ∈ set (enumR as s kk)" by blast
+      and mem: "Lval_at as s oL jL \<in> set (enumR as s kk)" by blast
     then obtain jR where jR: "jR < length (enumR as s kk)"
       and eq:  "Lval_at as s oL jL = enumR as s kk ! jR"
       using in_set_conv_nth by metis
@@ -1397,15 +1397,15 @@ proof -
     case True
     (* by uniqueness, no other j' witnesses baseline *)
     have no_other:
-      "⋀j'. j' < length (enumL as s kk) ⟹ j' ≠ j ⟹
-         Lval_at as s ((!) (x0 as s)) j' ∉ set (enumR as s kk)"
+      "\<And>j'. j' < length (enumL as s kk) \<Longrightarrow> j' \<noteq> j \<Longrightarrow>
+         Lval_at as s ((!) (x0 as s)) j' \<notin> set (enumR as s kk)"
       using baseline_only_j True by blast
 
-    have not_good_out: "¬ good as s oL_out ((!) (x0 as s))"
+    have not_good_out: "\<not> good as s oL_out ((!) (x0 as s))"
     proof
       assume H: "good as s oL_out ((!) (x0 as s))"
       then obtain j' where j'lt: "j' < length (enumL as s kk)"
-        and mem': "Lval_at as s oL_out j' ∈ set (enumR as s kk)"
+        and mem': "Lval_at as s oL_out j' \<in> set (enumR as s kk)"
         by (auto simp: Good_char)
       show False
       proof (cases "j' = j")
@@ -1414,13 +1414,13 @@ proof -
         using mem' by blast
       next
         case False
-        have "Lval_at as s ((!) (x0 as s)) j' ∈ set (enumR as s kk)"
+        have "Lval_at as s ((!) (x0 as s)) j' \<in> set (enumR as s kk)"
           using same_block[OF False] mem' by simp
         with no_other[OF j'lt False] show False by contradiction
       qed
     qed
 
-    have outside_out: "∀i. i ∉ blockL_abs enc0 as s j ⟶ oL_out i = (x0 as s) ! i"
+    have outside_out: "\<forall>i. i \<notin> blockL_abs enc0 as s j \<longrightarrow> oL_out i = (x0 as s) ! i"
       by (simp add: oL_out_def)
 
     show ?thesis
@@ -1432,7 +1432,7 @@ proof -
     have good_in': "good as s oL_in ((!) (x0 as s))"
       using Good_char jL Lval_in v_inR by blast
 
-    have outside_in: "∀i. i ∉ blockL_abs enc0 as s j ⟶ oL_in i = (x0 as s) ! i"
+    have outside_in: "\<forall>i. i \<notin> blockL_abs enc0 as s j \<longrightarrow> oL_in i = (x0 as s) ! i"
       by (simp add: oL_in_def)
 
     show ?thesis
@@ -1442,18 +1442,18 @@ qed
 
 lemma run_agrees_on_seen:
   fixes T :: "('i,'j) dtr"
-  assumes L: "⋀i. i ∈ seenL_run oL oR T ⟹ oL i = oL' i"
-      and R: "⋀j. j ∈ seenR_run oL oR T ⟹ oR j = oR' j"
+  assumes L: "\<And>i. i \<in> seenL_run oL oR T \<Longrightarrow> oL i = oL' i"
+      and R: "\<And>j. j \<in> seenR_run oL oR T \<Longrightarrow> oR j = oR' j"
   shows "run oL oR T = run oL' oR' T"
   using L R by (induction T) auto
 
 lemma flipR_pointwise_block:
-  fixes oL oR :: "nat ⇒ bool" and j :: nat
+  fixes oL oR :: "nat \<Rightarrow> bool" and j :: nat
   assumes jR: "j < length (enumR as s kk)"
-      and R2: "2 ≤ length (enumR as s kk)"
-  shows "∃oR'.
-           (∀i. i ∉ blockR_abs enc0 as s kk j ⟶ oR' i = oR i)
-         ∧ Rval_at as s oR' j ≠ Rval_at as s oR j"
+      and R2: "2 \<le> length (enumR as s kk)"
+  shows "\<exists>oR'.
+           (\<forall>i. i \<notin> blockR_abs enc0 as s kk j \<longrightarrow> oR' i = oR i)
+         \<and> Rval_at as s oR' j \<noteq> Rval_at as s oR j"
 proof -
   (* pick two different catalog values from enumR *)
   have len1: "1 < length (enumR as s kk)" using R2 by simp
@@ -1461,14 +1461,14 @@ proof -
   define u where "u = enumR as s kk ! 0"
   define v where "v = enumR as s kk ! 1"
 
-  have u_in: "u ∈ set (enumR as s kk)"
+  have u_in: "u \<in> set (enumR as s kk)"
     unfolding u_def nth_mem R2 by (meson len1 nth_mem order.strict_trans zero_less_one)
-  have v_in: "v ∈ set (enumR as s kk)"
+  have v_in: "v \<in> set (enumR as s kk)"
     unfolding v_def by (meson len1 nth_mem order.strict_trans zero_less_one)
 
   have distinct_enumR: "distinct (enumR as s kk)"
     by (simp add: enumR_def)  (* sorted_list_of_set -> distinct *)
-  have uv_ne: "u ≠ v"
+  have uv_ne: "u \<noteq> v"
     using distinct_enumR R2 len1 distinct_conv_nth
     unfolding u_def v_def
     by (metis length_pos_if_in_set u_in zero_neq_one)
@@ -1484,9 +1484,9 @@ proof -
 
   (* overwrite the whole j-th R block with bits for v *)
   define oR' where
-    "oR' i = (if ?a ≤ i ∧ i < ?a + ?w then bv ! (i - ?a) else oR i)" for i
+    "oR' i = (if ?a \<le> i \<and> i < ?a + ?w then bv ! (i - ?a) else oR i)" for i
 
-  have outside_eq: "⋀i. i ∉ blockR_abs enc0 as s kk j ⟹ oR' i = oR i"
+  have outside_eq: "\<And>i. i \<notin> blockR_abs enc0 as s kk j \<Longrightarrow> oR' i = oR i"
     by (auto simp: oR'_def blockR_abs_def)
 
   (* slice [a ..< a+w] becomes exactly bv under oR' *)
@@ -1499,7 +1499,7 @@ proof -
     hence iw: "i < ?w" by simp
     have idx: "[?a ..< ?a + ?w] ! i = ?a + i"
       using iw by simp
-    have inblk: "?a ≤ ?a + i ∧ ?a + i < ?a + ?w"
+    have inblk: "?a \<le> ?a + i \<and> ?a + i < ?a + ?w"
       using iw by simp
     show "map oR' [?a ..< ?a + ?w] ! i = bv ! i"
       using nth_map idx oR'_def inblk by simp
@@ -1509,7 +1509,7 @@ proof -
     by (simp add: Rval_at_def slice_bv bv_val)
 
   (* either we already differ from v, or we first overwrite to u, which differs from v *)
-  consider (diff) "Rval_at as s oR j ≠ v" | (eqv) "Rval_at as s oR j = v" by blast
+  consider (diff) "Rval_at as s oR j \<noteq> v" | (eqv) "Rval_at as s oR j = v" by blast
   then show ?thesis
   proof cases
     case diff
@@ -1518,7 +1518,7 @@ proof -
     case eqv
     (* overwrite to u to force a difference *)
     define oR_u where
-      "oR_u i = (if ?a ≤ i ∧ i < ?a + ?w then bu ! (i - ?a) else oR i)" for i
+      "oR_u i = (if ?a \<le> i \<and> i < ?a + ?w then bu ! (i - ?a) else oR i)" for i
     have slice_bu: "map oR_u [?a ..< ?a + ?w] = bu"
     proof (rule nth_equalityI)
       show "length (map oR_u [?a ..< ?a + ?w]) = length bu"
@@ -1528,23 +1528,23 @@ proof -
       hence iw: "i < ?w" by simp
       have idx: "[?a ..< ?a + ?w] ! i = ?a + i"
         using iw by simp
-      have inblk: "?a ≤ ?a + i ∧ ?a + i < ?a + ?w"
+      have inblk: "?a \<le> ?a + i \<and> ?a + i < ?a + ?w"
         using iw by simp
       show "map oR_u [?a ..< ?a + ?w] ! i = bu ! i"
         using nth_map idx oR_u_def inblk by simp
     qed
     have old_to_u: "Rval_at as s oR_u j = u"
       by (simp add: Rval_at_def slice_bu bu_val)
-    have diff_now: "Rval_at as s oR_u j ≠ Rval_at as s oR j"
+    have diff_now: "Rval_at as s oR_u j \<noteq> Rval_at as s oR j"
       using eqv old_to_u uv_ne by simp
-    have outside_eq_u: "∀i. i ∉ blockR_abs enc0 as s kk j ⟶ oR_u i = oR i"
+    have outside_eq_u: "\<forall>i. i \<notin> blockR_abs enc0 as s kk j \<longrightarrow> oR_u i = oR i"
       by (simp add: oR_u_def blockR_abs_def)
     from outside_eq_u diff_now show ?thesis by blast
   qed
 qed
 
-definition L0 where "L0 as s = Lset as s ∪ Rset as s"
-definition R0 where "R0 as s = Lset as s ∪ Rset as s"
+definition L0 where "L0 as s = Lset as s \<union> Rset as s"
+definition R0 where "R0 as s = Lset as s \<union> Rset as s"
 definition T0 where
   "T0 as s =
      tm_to_dtr' head0 stepf final_acc
@@ -1555,14 +1555,14 @@ definition Good where "Good as s = good as s"
 lemma seenL_T0_subset_read0:
   fixes x :: "bool list"
   assumes X: "x = enc as s kk"
-  shows "seenL_run ((!) x) ((!) y) (T0 as s) ⊆ Base.read0 M x"
+  shows "seenL_run ((!) x) ((!) y) (T0 as s) \<subseteq> Base.read0 M x"
 proof -
   let ?T = "tm_to_dtr' head0 stepf final_acc (steps M x) (conf M x 0)"
   have T0_eq: "T0 as s = ?T" by (simp add: T0_def X)
   have "seenL_run ((!) x) ((!) y) ?T
-          ⊆ (λu. nat (head0 (drive u (conf M x 0) ((!) x)))) ` {..< steps M x}"
+          \<subseteq> (\<lambda>u. nat (head0 (drive u (conf M x 0) ((!) x)))) ` {..< steps M x}"
     by (rule seenL_tm_to_dtr_subset_read0_helper)
-  also have "... = (λu. nat (head0 (conf M x u))) ` {..< steps M x}"
+  also have "... = (\<lambda>u. nat (head0 (conf M x u))) ` {..< steps M x}"
     by (simp add: drive_conf)
   also have "... = Base.read0 M x"
     by (simp add: Base.read0_def)
@@ -1572,14 +1572,14 @@ qed
 lemma seenR_T0_subset_read0:
   fixes x :: "bool list"
   assumes X: "x = enc as s kk"
-  shows "seenR_run ((!) x) ((!) y) (T0 as s) ⊆ Base.read0 M x"
+  shows "seenR_run ((!) x) ((!) y) (T0 as s) \<subseteq> Base.read0 M x"
 proof -
   let ?T = "tm_to_dtr' head0 stepf final_acc (steps M x) (conf M x 0)"
   have T0_eq: "T0 as s = ?T" by (simp add: T0_def X)
   have "seenR_run ((!) x) ((!) y) ?T
-          ⊆ (λu. nat (head0 (drive u (conf M x 0) ((!) x)))) ` {..< steps M x}"
+          \<subseteq> (\<lambda>u. nat (head0 (drive u (conf M x 0) ((!) x)))) ` {..< steps M x}"
     by (rule seenR_tm_to_dtr_subset_read0_helper)
-  also have "... = (λu. nat (head0 (conf M x u))) ` {..< steps M x}"
+  also have "... = (\<lambda>u. nat (head0 (conf M x u))) ` {..< steps M x}"
     by (simp add: drive_conf)
   also have "... = Base.read0 M x"
     by (simp add: Base.read0_def)
@@ -1609,9 +1609,9 @@ qed
 
 lemma Good_char_encL:
   "Good as s ((!) (x0 as s)) oR
-   ⟷ (∃jR<length (enumR as s kk). Rval_at as s oR jR ∈ set (enumL as s kk))"
+   \<longleftrightarrow> (\<exists>jR<length (enumR as s kk). Rval_at as s oR jR \<in> set (enumL as s kk))"
 proof
-  (* ⇒ *)
+  (* \<Rightarrow> *)
   assume G: "Good as s ((!) (x0 as s)) oR"
   then obtain jL jR
     where jL: "jL < length (enumL as s kk)"
@@ -1620,15 +1620,15 @@ proof
     unfolding Good_def good_def by blast
   have "Rval_at as s oR jR = enumL as s kk ! jL"
     using Eq by (simp add: Lval_at_on_enc_block jL)
-  hence "Rval_at as s oR jR ∈ set (enumL as s kk)"
+  hence "Rval_at as s oR jR \<in> set (enumL as s kk)"
     using jL in_set_conv_nth by metis
-  thus "∃jR<length (enumR as s kk). Rval_at as s oR jR ∈ set (enumL as s kk)"
+  thus "\<exists>jR<length (enumR as s kk). Rval_at as s oR jR \<in> set (enumL as s kk)"
     using jR by blast
-  (* ⇐ *)
+  (* \<Leftarrow> *)
 next
-  assume Ex: "∃jR<length (enumR as s kk). Rval_at as s oR jR ∈ set (enumL as s kk)"
+  assume Ex: "\<exists>jR<length (enumR as s kk). Rval_at as s oR jR \<in> set (enumL as s kk)"
   then obtain jR where jR: "jR < length (enumR as s kk)"
-    and Mem: "Rval_at as s oR jR ∈ set (enumL as s kk)" by blast
+    and Mem: "Rval_at as s oR jR \<in> set (enumL as s kk)" by blast
   then obtain jL where jL: "jL < length (enumL as s kk)"
     and Nth: "enumL as s kk ! jL = Rval_at as s oR jR"
     by (meson in_set_conv_nth)
@@ -1642,9 +1642,9 @@ qed
 
 lemma Good_char_encR:
   "Good as s oL ((!) (x0 as s))
-   ⟷ (∃jL<length (enumL as s kk). Lval_at as s oL jL ∈ set (enumR as s kk))"
+   \<longleftrightarrow> (\<exists>jL<length (enumL as s kk). Lval_at as s oL jL \<in> set (enumR as s kk))"
 proof
-  (* ⇒ *)
+  (* \<Rightarrow> *)
   assume H: "Good as s oL ((!) (x0 as s))"
   then obtain jL jR where
     jL: "jL < length (enumL as s kk)" and jR: "jR < length (enumR as s kk)" and
@@ -1652,13 +1652,13 @@ proof
     unfolding Good_def good_def by blast
   hence "Lval_at as s oL jL = enumR as s kk ! jR"
     by (simp add: Rval_at_on_enc_block jR)
-  thus "∃jL<length (enumL as s kk). Lval_at as s oL jL ∈ set (enumR as s kk)"
+  thus "\<exists>jL<length (enumL as s kk). Lval_at as s oL jL \<in> set (enumR as s kk)"
     using jL in_set_conv_nth by (metis jR)
 next
-  (* ⇐ *)
-  assume "∃jL<length (enumL as s kk). Lval_at as s oL jL ∈ set (enumR as s kk)"
+  (* \<Leftarrow> *)
+  assume "\<exists>jL<length (enumL as s kk). Lval_at as s oL jL \<in> set (enumR as s kk)"
   then obtain jL where jL: "jL < length (enumL as s kk)"
-    and mem: "Lval_at as s oL jL ∈ set (enumR as s kk)" by blast
+    and mem: "Lval_at as s oL jL \<in> set (enumR as s kk)" by blast
   then obtain jR where jR: "jR < length (enumR as s kk)"
     and eq0: "enumR as s kk ! jR = Lval_at as s oL jL"
     using in_set_conv_nth by metis
@@ -1670,17 +1670,17 @@ qed
 
 lemma flipL0:
   assumes jL: "j < length (enumL as s kk)"
-      and L2: "2 ≤ length (enumL as s kk)"
-      and hit:  "∃v∈set (enumL as s kk). v ∈ set (enumR as s kk)"
-      and miss: "∃v∈set (enumL as s kk). v ∉ set (enumR as s kk)"
+      and L2: "2 \<le> length (enumL as s kk)"
+      and hit:  "\<exists>v\<in>set (enumL as s kk). v \<in> set (enumR as s kk)"
+      and miss: "\<exists>v\<in>set (enumL as s kk). v \<notin> set (enumR as s kk)"
       and baseline_only_j:
-        "Good as s ((!) (x0 as s)) ((!) (x0 as s)) ⟶
-        (∀j'<length (enumL as s kk). j' ≠ j ⟶
-        Lval_at as s ((!) (x0 as s)) j' ∉ set (enumR as s kk))"
-  shows "∃oL'.
-           (∀i. i ∉ blockL_abs enc0 as s j ⟶ oL' i = ((!) (enc as s kk)) i)
-         ∧ Good as s oL' ((!) (enc as s kk))
-           ≠ Good as s ((!) (enc as s kk)) ((!) (enc as s kk))"
+        "Good as s ((!) (x0 as s)) ((!) (x0 as s)) \<longrightarrow>
+        (\<forall>j'<length (enumL as s kk). j' \<noteq> j \<longrightarrow>
+        Lval_at as s ((!) (x0 as s)) j' \<notin> set (enumR as s kk))"
+  shows "\<exists>oL'.
+           (\<forall>i. i \<notin> blockL_abs enc0 as s j \<longrightarrow> oL' i = ((!) (enc as s kk)) i)
+         \<and> Good as s oL' ((!) (enc as s kk))
+           \<noteq> Good as s ((!) (enc as s kk)) ((!) (enc as s kk))"
 proof -
   let ?a = "length (enc0 as s) + offL as s j"
   let ?w = "W as s"
@@ -1689,9 +1689,9 @@ proof -
     using L2 by auto
   define p where "p = enumL as s kk ! 0"
   define q where "q = enumL as s kk ! 1"
-  have p_in: "p ∈ set (enumL as s kk)"
+  have p_in: "p \<in> set (enumL as s kk)"
     unfolding p_def by (rule nth_mem) (use lt0 in simp)
-  have q_in: "q ∈ set (enumL as s kk)"
+  have q_in: "q \<in> set (enumL as s kk)"
     unfolding q_def by (rule nth_mem) (use lt1 in simp)
   obtain bp where bp_len: "length bp = ?w" and bp_val: "from_bits bp = p"
     using p_in bits_roundtrip by blast
@@ -1700,10 +1700,10 @@ proof -
 
   (* two candidate left-oracles that overwrite only block j *)
   define oL_p where
-    "oL_p i = (if i ∈ blockL_abs enc0 as s j then bp ! (i - ?a)
+    "oL_p i = (if i \<in> blockL_abs enc0 as s j then bp ! (i - ?a)
                else (enc as s kk) ! i)" for i
   define oL_q where
-    "oL_q i = (if i ∈ blockL_abs enc0 as s j then bq ! (i - ?a)
+    "oL_q i = (if i \<in> blockL_abs enc0 as s j then bq ! (i - ?a)
                else (enc as s kk) ! i)" for i
   have blk_eq: "blockL_abs enc0 as s j = {?a ..< ?a + ?w}"
     by (simp add: blockL_abs_def offL_def)
@@ -1718,7 +1718,7 @@ proof -
       fix t assume "t < length (map oL_p [?a ..< ?a + ?w])"
       hence tw: "t < ?w" by simp
       have idx: "[?a ..< ?a + ?w] ! t = ?a + t" using tw by simp
-      have inblk: "?a + t ∈ blockL_abs enc0 as s j"
+      have inblk: "?a + t \<in> blockL_abs enc0 as s j"
         using tw by (simp add: blk_eq)
       show "map oL_p [?a ..< ?a + ?w] ! t = bp ! t"
         using nth_map idx oL_p_def inblk by (simp add: tw)
@@ -1737,7 +1737,7 @@ proof -
       fix t assume "t < length (map oL_q [?a ..< ?a + ?w])"
       hence tw: "t < ?w" by simp
       have idx: "[?a ..< ?a + ?w] ! t = ?a + t" using tw by simp
-      have inblk: "?a + t ∈ blockL_abs enc0 as s j"
+      have inblk: "?a + t \<in> blockL_abs enc0 as s j"
         using tw by (simp add: blk_eq)
       show "map oL_q [?a ..< ?a + ?w] ! t = bq ! t"
         using nth_map idx oL_q_def inblk by (simp add: tw)
@@ -1747,23 +1747,23 @@ proof -
   qed
 
   have outside_p:
-    "∀i. i ∉ blockL_abs enc0 as s j ⟶ oL_p i = (enc as s kk) ! i"
+    "\<forall>i. i \<notin> blockL_abs enc0 as s j \<longrightarrow> oL_p i = (enc as s kk) ! i"
     by (simp add: oL_p_def)
   have outside_q:
-    "∀i. i ∉ blockL_abs enc0 as s j ⟶ oL_q i = (enc as s kk) ! i"
+    "\<forall>i. i \<notin> blockL_abs enc0 as s j \<longrightarrow> oL_q i = (enc as s kk) ! i"
     by (simp add: oL_q_def)
 
   (* Decide which one flips relative to the baseline *)
   show ?thesis
-  proof (cases "Good as s (λi. (enc as s kk) ! i) (λi. (enc as s kk) ! i)")
+  proof (cases "Good as s (\<lambda>i. (enc as s kk) ! i) (\<lambda>i. (enc as s kk) ! i)")
     case True
-    (* Baseline is good → pick an L-value outside set(enumR) to force ¬Good *)
-    from miss obtain v_out where v_outL: "v_out ∈ set (enumL as s kk)"
-      and v_outNR: "v_out ∉ set (enumR as s kk)" by blast
+    (* Baseline is good \<rightarrow> pick an L-value outside set(enumR) to force \<not>Good *)
+    from miss obtain v_out where v_outL: "v_out \<in> set (enumL as s kk)"
+      and v_outNR: "v_out \<notin> set (enumR as s kk)" by blast
     obtain bv where bv_len: "length bv = ?w" and bv_val: "from_bits bv = v_out"
       using v_outL bits_roundtrip by blast
     define oL_out where
-      "oL_out i = (if i ∈ blockL_abs enc0 as s j then bv ! (i - ?a)
+      "oL_out i = (if i \<in> blockL_abs enc0 as s j then bv ! (i - ?a)
                    else (enc as s kk) ! i)" for i
     have Lval_out: "Lval_at as s oL_out j = v_out"
     proof -
@@ -1780,7 +1780,7 @@ proof -
         fix t assume "t < length (map oL_out [?a ..< ?a + ?w])"
         hence tw: "t < ?w" by simp
         have idx: "[?a ..< ?a + ?w] ! t = ?a + t" using tw by simp
-        have inblk: "?a + t ∈ blockL_abs enc0 as s j"
+        have inblk: "?a + t \<in> blockL_abs enc0 as s j"
           using tw by (simp add: blk_eq)
         show "map oL_out [?a ..< ?a + ?w] ! t = bv ! t"
           using nth_map idx oL_out_def inblk by (simp add: tw)
@@ -1791,9 +1791,9 @@ proof -
     qed
 
     have same_block:
-      "⋀j'. j' ≠ j ⟹ Lval_at as s oL_out j' = Lval_at as s ((!) (x0 as s)) j'"
+      "\<And>j'. j' \<noteq> j \<Longrightarrow> Lval_at as s oL_out j' = Lval_at as s ((!) (x0 as s)) j'"
     proof -
-      fix j' assume ne: "j' ≠ j"
+      fix j' assume ne: "j' \<noteq> j"
       let ?a' = "length (enc0 as s) + offL as s j'"
       let ?w' = "W as s"
       have blk': "blockL_abs enc0 as s j' = {?a' ..< ?a' + ?w'}"
@@ -1808,8 +1808,8 @@ proof -
         fix t assume "t < length (map oL_out [?a' ..< ?a' + ?w'])"
         hence tw: "t < ?w'" by simp
         have idx: "[?a' ..< ?a' + ?w'] ! t = ?a' + t" using tw by simp
-        have in_j': "?a' + t ∈ blockL_abs enc0 as s j'" using tw by (simp add: blk')
-        have not_in_j: "?a' + t ∉ blockL_abs enc0 as s j"
+        have in_j': "?a' + t \<in> blockL_abs enc0 as s j'" using tw by (simp add: blk')
+        have not_in_j: "?a' + t \<notin> blockL_abs enc0 as s j"
           using blockL_abs_disjoint[OF ne] in_j' by auto
         have out_eq: "oL_out (?a' + t) = (x0 as s) ! (?a' + t)"
           by (simp add: oL_out_def not_in_j)
@@ -1823,18 +1823,18 @@ proof -
      (* Good characterization specialized to oL_out *)
     have Good_char_oL_out:
       "Good as s oL_out ((!) (x0 as s))
-       ⟷ (∃jL<length (enumL as s kk). Lval_at as s oL_out jL ∈ set (enumR as s kk))"
+       \<longleftrightarrow> (\<exists>jL<length (enumL as s kk). Lval_at as s oL_out jL \<in> set (enumR as s kk))"
       by (rule Good_char_encR)
 
-    (* no jL witnesses after the overwrite ⇒ ¬Good *)
-    have not_good_out: "¬ Good as s oL_out ((!) (x0 as s))"
+    (* no jL witnesses after the overwrite \<Rightarrow> \<not>Good *)
+    have not_good_out: "\<not> Good as s oL_out ((!) (x0 as s))"
     proof -
       have none:
-        "⋀j'. j' < length (enumL as s kk) ⟹
-          Lval_at as s oL_out j' ∉ set (enumR as s kk)"
+        "\<And>j'. j' < length (enumL as s kk) \<Longrightarrow>
+          Lval_at as s oL_out j' \<notin> set (enumR as s kk)"
       proof -
         fix j' assume j'lt: "j' < length (enumL as s kk)"
-        show "Lval_at as s oL_out j' ∉ set (enumR as s kk)"
+        show "Lval_at as s oL_out j' \<notin> set (enumR as s kk)"
         proof (cases "j' = j")
           case True
           have "Lval_at as s oL_out j' = v_out"
@@ -1844,29 +1844,29 @@ proof -
           case False
           have "Lval_at as s oL_out j' = Lval_at as s ((!) (x0 as s)) j'"
             by (rule same_block[OF False])
-          also have "... ∉ set (enumR as s kk)"
-            using baseline_only_j ‹Good as s ((!) (x0 as s)) ((!) (x0 as s))› j'lt False by blast
+          also have "... \<notin> set (enumR as s kk)"
+            using baseline_only_j \<open>Good as s ((!) (x0 as s)) ((!) (x0 as s))\<close> j'lt False by blast
           finally show ?thesis .
         qed
       qed
       thus ?thesis by (simp only: Good_char_oL_out) blast
     qed
 
-    have outside_out: "∀i. i ∉ blockL_abs enc0 as s j ⟶ oL_out i = (x0 as s) ! i"
+    have outside_out: "\<forall>i. i \<notin> blockL_abs enc0 as s j \<longrightarrow> oL_out i = (x0 as s) ! i"
       by (simp add: oL_out_def)
     show ?thesis
       by (intro exI[of _ oL_out]) (use outside_out True not_good_out in auto)
 
   next
     case False
-    (* Baseline is NOT good → choose an L-value that *is* in enumR to force Good *)
-    from hit obtain v_in where v_inL: "v_in ∈ set (enumL as s kk)"
-      and v_inR: "v_in ∈ set (enumR as s kk)" by blast
+    (* Baseline is NOT good \<rightarrow> choose an L-value that *is* in enumR to force Good *)
+    from hit obtain v_in where v_inL: "v_in \<in> set (enumL as s kk)"
+      and v_inR: "v_in \<in> set (enumR as s kk)" by blast
     obtain bv where bv_len: "length bv = ?w" and bv_val: "from_bits bv = v_in"
       using v_inL bits_roundtrip by blast
 
     define oL_in where
-      "oL_in i = (if i ∈ blockL_abs enc0 as s j then bv ! (i - ?a)
+      "oL_in i = (if i \<in> blockL_abs enc0 as s j then bv ! (i - ?a)
                   else (x0 as s) ! i)" for i
 
     have blk_eq': "blockL_abs enc0 as s j = {?a ..< ?a + ?w}"
@@ -1879,7 +1879,7 @@ proof -
       fix t assume "t < length (map oL_in [?a ..< ?a + ?w])"
       hence tw: "t < ?w" by simp
       have idx: "[?a ..< ?a + ?w] ! t = ?a + t" using tw by simp
-      have inblk: "?a + t ∈ blockL_abs enc0 as s j" using tw by (simp add: blk_eq')
+      have inblk: "?a + t \<in> blockL_abs enc0 as s j" using tw by (simp add: blk_eq')
       show "map oL_in [?a ..< ?a + ?w] ! t = bv ! t"
         using nth_map idx oL_in_def inblk by (simp add: tw)
     qed
@@ -1890,7 +1890,7 @@ proof -
     have good_in: "Good as s oL_in ((!) (x0 as s))"
       using Good_char_encR Lval_in v_inR jL by auto
 
-    have outside_in: "∀i. i ∉ blockL_abs enc0 as s j ⟶ oL_in i = (x0 as s) ! i"
+    have outside_in: "\<forall>i. i \<notin> blockL_abs enc0 as s j \<longrightarrow> oL_in i = (x0 as s) ! i"
       by (simp add: oL_in_def)
 
     show ?thesis
@@ -1912,66 +1912,199 @@ proof -
 
   have RUN0:
     "final_acc (drive (steps M ?x) (conf M ?x 0) oL) = run oL ((!) ?x) ?T"
-      by (simp add: run_drive_T0)
+    by (simp add: run_drive_T0)
 
-  define may_read where "may_read ≡ Lset as s ∪ Rset as s"
-  define Y where "Y i = (if i ∈ may_read then oL i else ?x ! i)" for i
+  define may_read :: "nat set"
+    where "may_read \<equiv> Lset as s \<union> Rset as s"
+
+  define Y :: "nat \<Rightarrow> bool"
+    where "Y i = (if i \<in> may_read then oL i else (x0 as s) ! i)"
   define y where "y = map Y [0..<length ?x]"
-  have len_y[simp]: "length y = length ?x" by (simp add: y_def)
+  define yL :: "bool list"
+    where "yL = map Y [0..<length (x0 as s)]"
 
   have SL_sub_read0:
-    "seenL_run ((!) y) ((!) ?x) ?T ⊆ Base.read0 M ?x"
-    by (rule seenL_T0_subset_read0) (simp add: x0_is_enc)
+  "seenL_run ((!) ?x) ((!) y) (T0 as s) \<subseteq> Base.read0 M ?x"
+    using seenL_T0_subset_read0[where x="?x" and y=y]
+    by simp
+
+  have len_x[simp]:
+  "length ?x = length (enc0 as s) + length (padL as s kk) + length (padR as s kk)"
+    by (simp add: enc_def)
+
   have read0_sub_may:
-    "Base.read0 M ?x ⊆ may_read"
+    "Base.read0 M ?x \<subseteq> may_read"
     unfolding may_read_def by (rule read0_subset_blocks_abs)
 
+  have may_read_lt_len:
+  "\<And>i. i \<in> may_read \<Longrightarrow> i < length ?x"
+  proof -
+    fix i assume "i \<in> may_read"
+    hence "i \<in> Lset as s \<or> i \<in> Rset as s" by (simp add: may_read_def)
+    then consider
+      (L) j where "j < length (enumL as s kk)" and "i \<in> blockL_abs enc0 as s j"
+    | (R) j where "j < length (enumR as s kk)" and "i \<in> blockR_abs enc0 as s kk j"
+      unfolding Lset_def Rset_def by auto
+    thus "i < length ?x"
+    proof cases
+      case (L j)
+      let ?a = "length (enc0 as s) + offL as s j"
+      let ?w = "W as s"
+      have blk: "blockL_abs enc0 as s j = {?a ..< ?a + ?w}"
+        by (simp add: blockL_abs_def offL_def)
+      have top: "?a + ?w \<le> length ?x"
+        using offL_window_in_enc[OF L(1)] by simp
+      from L(2) have "i \<in> {?a ..< ?a + ?w}" by (simp add: blk)
+      then have "i < ?a + ?w" by simp   (* membership \<Rightarrow> upper bound *)
+      with top show ?thesis by linarith
+    next
+      case (R j)
+      let ?a = "length (enc0 as s) + offR as s kk j"
+      let ?w = "W as s"
+      have blk: "blockR_abs enc0 as s kk j = {?a ..< ?a + ?w}"
+        by (simp add: blockR_abs_def)
+      have top: "?a + ?w \<le> length ?x"
+        using offR_window_in_enc[OF R(1)] length_padL by simp
+      from R(2) have "i \<in> {?a ..< ?a + ?w}" by (simp add: blk)
+      then have "i < ?a + ?w" by simp
+      with top show ?thesis by linarith
+    qed
+  qed
+
   have agree_on_seenL:
-    "⋀i. i ∈ seenL_run ((!) y) ((!) ?x) ?T ⟹ (!) y i = oL i"
-    by (simp add: y_def Y_def SL_sub_read0 read0_sub_may)
+    "\<And>i. i \<in> seenL_run ((!) ?x) ((!) y) ?T \<Longrightarrow> y ! i = oL i"
+  proof -
+    fix i assume iSL: "i \<in> seenL_run ((!) ?x) ((!) y) ?T"
+    from SL_sub_read0 iSL have iR0: "i \<in> Base.read0 M ?x" by blast
+    from read0_sub_may iR0 have iMay: "i \<in> may_read" by blast
+    from may_read_lt_len iMay have iLt: "i < length ?x" .
+    have "y ! i = (map Y [0..<length ?x]) ! i" by (simp add: y_def)
+    also from iLt have "... = Y i" by simp
+    also from iMay have "... = oL i"
+      by (simp add: \<open>Y \<equiv> \<lambda>i. if i \<in> may_read then oL i else x0 as s ! i\<close>)
+    finally show "y ! i = oL i" .
+  qed
 
   have Good_normalize:
-    "Good as s ((!) y) ((!) ?x) = Good as s oL ((!) ?x)"
+  "Good as s ((!) y) ((!) ?x) = Good as s oL ((!) ?x)"
   proof -
     have Lwin_eq:
-      "⋀j. j < length (enumL as s kk) ⟹
-           Lval_at as s ((!) y) j = Lval_at as s oL j"
+      "\<And>j. j < length (enumL as s kk) \<Longrightarrow>
+         Lval_at as s ((!) y) j = Lval_at as s oL j"
     proof -
       fix j assume jL: "j < length (enumL as s kk)"
       let ?a = "length (enc0 as s) + offL as s j"
       let ?w = "W as s"
       have blk: "blockL_abs enc0 as s j = {?a ..< ?a + ?w}"
         by (simp add: blockL_abs_def offL_def)
+
+    (* the left block window lies within the length of ?x *)
+      have ALe: "?a + ?w \<le> length ?x"
+        using offL_window_in_enc[OF jL] by simp
+
       have slice_eq:
         "map ((!) y) [?a ..< ?a + ?w] = map oL [?a ..< ?a + ?w]"
       proof (rule nth_equalityI)
-        show "length (map ((!) y) [?a..< ?a+?w]) = length (map oL [?a..< ?a+?w])"
-          by simp
+        show "length (map ((!) y) [?a..< ?a+?w]) =
+            length (map oL       [?a..< ?a+?w])" by simp
       next
         fix t assume "t < length (map ((!) y) [?a..< ?a+?w])"
         then have tw: "t < ?w" by simp
         have idx: "[?a..< ?a+?w] ! t = ?a + t" using tw by simp
-        have in_may:
-          "?a + t ∈ may_read"
-          unfolding may_read_def
-          by (intro UnI1) (simp add: Lset_def blockL_abs_def UN_iff jL)
-        show "map ((!) y) [?a..< ?a+?w] ! t = map oL [?a..< ?a+?w] ! t"
-          by (simp add: idx y_def Y_def in_may)
+
+      (* index is inside [0..<length ?x] so we can index `y = map Y [0..<length ?x]` *)
+        have AT: "?a + t < length ?x" using ALe tw by linarith
+
+      (* show (?a + t) \<in> Lset, hence in may_read *)
+        have in_Lset: "?a + t \<in> Lset as s"
+        proof -
+          have mem: "?a + t \<in> blockL_abs enc0 as s j"
+            using tw by (simp add: blk)
+          have fam: "blockL_abs enc0 as s j
+               \<in> (blockL_abs enc0 as s ` {..<length (enumL as s kk)})"
+            using jL by (intro imageI) simp
+          show ?thesis
+            unfolding Lset_def
+            by (rule UnionI[OF fam mem])
+        qed
+        have in_may: "?a + t \<in> may_read"
+          unfolding may_read_def by (intro UnI1) (simp add: in_Lset)
+
+      (* left nth equals oL (?a+t) *)
+        have left: "map ((!) y) [?a..<?a+?w] ! t = oL (?a + t)"
+        proof -
+          (* push (!) y through the map; nth_map needs t < length [...], i.e. t < ?w *)
+          have A0: "map ((!) y) [?a..<?a+?w] ! t = (!) y ([?a..<?a+?w] ! t)"
+            using tw by simp
+          have A1: "[?a..<?a+?w] ! t = ?a + t"
+            using tw by simp
+
+  (* turn y!(?a+t) into Y (?a+t); nth_map+nth_upt need (?a+t) < length ?x, i.e. AT *)
+          have A2: "y ! (?a + t) = Y (?a + t)"
+            using AT by (simp add: y_def)
+
+  (* unfold Y and use the membership we already proved *)
+          have A3: "Y (?a + t) = (if (?a + t) \<in> may_read then oL (?a + t) else ?x ! (?a + t))"
+            by (simp add: \<open>Y \<equiv> \<lambda>i. if i \<in> may_read then oL i else x0 as s ! i\<close>)
+
+          from A0 A1 A2 A3 in_may
+          show ?thesis by simp
+        qed
+
+      (* right nth is also oL (?a+t) *)
+        have right: "map oL [?a..<?a+?w] ! t = oL (?a + t)"
+          using tw by (simp add: idx)
+
+        show "map ((!) y) [?a..< ?a+?w] ! t =
+            map oL       [?a..< ?a+?w] ! t"
+          using left right by simp
       qed
+
       show "Lval_at as s ((!) y) j = Lval_at as s oL j"
-        by (simp add: Lval_at_def slice_eq)
+      by (simp add: Lval_at_def slice_eq)
     qed
+
     show ?thesis
       unfolding Good_def good_def by (metis Lwin_eq)
+  qed
+
+  (* seen set for the base pair ((!) ?x, (!) ?x) is inside read0 M ?x *)
+(* left-seen set for ((!) y, (!) ?x) is within read0 on input y *)
+  have SL_sub_read0_yx:
+  "seenL_run ((!) y) ((!) (x0 as s)) (T0 as s) \<subseteq> Base.read0 M (x0 as s)"
+  by (rule seenL_T0_subset_read0[where x="x0 as s" and y=y])
+     (simp add: x0_def enc_def)
+
+(* any read0 is within Lset \<union> Rset (= may_read) *)
+  have read0_sub_may: "Base.read0 M ?x \<subseteq> may_read"
+    unfolding may_read_def by (rule read0_subset_blocks_abs)
+
+(* length alignment *)
+  have len_y[simp]: "length y = length ?x"
+    by (simp add: y_def)
+
+  have agree_on_seenL_for_pair:
+    "\<And>i. i \<in> seenL_run ((!) y) ((!) ?x) ?T \<Longrightarrow> (!) y i = oL i"
+  proof -
+    fix i assume iSL: "i \<in> seenL_run ((!) y) ((!) ?x) ?T"
+    from SL_sub_read0_yx iSL have iR0: "i \<in> Base.read0 M ?x" by blast
+    from read0_sub_may iR0 have iMay: "i \<in> may_read" by blast
+    have iLt: "i < length ?x" by (rule may_read_lt_len[OF iMay])
+    have "(!) y i = y ! i" by simp
+    also have "... = (map Y [0..<length ?x]) ! i" by (simp add: y_def)
+    also from iLt have "... = Y i" by simp
+    also from iMay have "... = oL i"
+      by (simp add: \<open>Y \<equiv> \<lambda>i. if i \<in> may_read then oL i else x0 as s ! i\<close>)
+    finally show "(!) y i = oL i" .
   qed
 
   have run_yx_eq_olx:
     "run ((!) y) ((!) ?x) ?T = run oL ((!) ?x) ?T"
   proof (rule run_agrees_on_seen)
-    show "⋀i. i ∈ seenL_run ((!) y) ((!) ?x) ?T ⟹ (!) y i = oL i"
-      by (rule agree_on_seenL)
+    show "\<And>i. i \<in> seenL_run ((!) y) ((!) ?x) ?T \<Longrightarrow> (!) y i = oL i"
+      by (rule agree_on_seenL_for_pair)
   next
-    show "⋀i. i ∈ seenR_run ((!) y) ((!) ?x) ?T ⟹ (!) ?x i = (!) ?x i"
+    show "\<And>i. i \<in> seenR_run ((!) y) ((!) ?x) ?T \<Longrightarrow> (!) ?x i = (!) ?x i"
       by simp
   qed
 
@@ -1980,21 +2113,21 @@ proof -
     by (rule correct_T0)
 
   have SL_sub_read0_x:
-    "seenL_run ((!) ?x) ((!) ?x) ?T ⊆ Base.read0 M ?x"
+    "seenL_run ((!) ?x) ((!) ?x) ?T \<subseteq> Base.read0 M ?x"
     by (rule seenL_T0_subset_read0) simp
 
   have run_yx_eq_xx:
     "run ((!) y) ((!) ?x) ?T = run ((!) ?x) ((!) ?x) ?T"
   proof (rule run_agrees_on_seen)
-    show "⋀i. i ∈ seenL_run ((!) y) ((!) ?x) ?T ⟹ (!) y i = (!) ?x i"
+    show "\<And>i. i \<in> seenL_run ((!) y) ((!) ?x) ?T \<Longrightarrow> (!) y i = (!) ?x i"
     proof -
-      fix i assume iSL: "i ∈ seenL_run ((!) y) ((!) ?x) ?T"
-      from SL_sub_read0 iSL have "i ∈ Base.read0 M ?x" by blast
-      with read0_sub_may have "i ∈ may_read" by blast
+      fix i assume iSL: "i \<in> seenL_run ((!) y) ((!) ?x) ?T"
+      from SL_sub_read0 iSL have "i \<in> Base.read0 M ?x" by blast
+      with read0_sub_may have "i \<in> may_read" by blast
       thus "(!) y i = (!) ?x i" by (simp add: y_def Y_def)
     qed
   next
-    show "⋀i. i ∈ seenR_run ((!) y) ((!) ?x) ?T ⟹ (!) ?x i = (!) ?x i" 
+    show "\<And>i. i \<in> seenR_run ((!) y) ((!) ?x) ?T \<Longrightarrow> (!) ?x i = (!) ?x i" 
       by simp
   qed
 
@@ -2006,8 +2139,6 @@ proof -
     by (rule run_xx_eq_Good_xx)
   also have "... = Good as s ((!) y) ((!) ?x)"
     by (simp add: Good_normalize[symmetric])
-  also have "... = Good as s ((!) y) ((!) ?x)"
-    by (simp add: Good_normalize)
   finally show ?thesis by (simp add: RUN0)
 qed
 
@@ -2022,27 +2153,27 @@ proof -
     "final_acc (drive (steps M ?x) (conf M ?x 0) ((!) ?x)) = run ((!) ?x) oR ?T"
     by (simp add: run_drive_T0)
 
-  define may_read where "may_read ≡ Lset as s ∪ Rset as s"
-  define Z where "Z i = (if i ∈ may_read then oR i else ?x ! i)" for i
+  define may_read where "may_read \<equiv> Lset as s \<union> Rset as s"
+  define Z where "Z i = (if i \<in> may_read then oR i else ?x ! i)" for i
   define z where "z = map Z [0..<length ?x]"
   have len_z[simp]: "length z = length ?x" by (simp add: z_def)
 
    have SR_sub_read0:
-    "seenR_run ((!) ?x) ((!) z) ?T ⊆ Base.read0 M ?x"
+    "seenR_run ((!) ?x) ((!) z) ?T \<subseteq> Base.read0 M ?x"
     by (rule seenR_T0_subset_read0) (simp add: x0_is_enc)
   have read0_sub_may:
-    "Base.read0 M ?x ⊆ may_read"
+    "Base.read0 M ?x \<subseteq> may_read"
     unfolding may_read_def by (rule read0_subset_blocks_abs)
 
   have agree_on_seenR:
-    "⋀i. i ∈ seenR_run ((!) ?x) ((!) z) ?T ⟹ (!) z i = oR i"
+    "\<And>i. i \<in> seenR_run ((!) ?x) ((!) z) ?T \<Longrightarrow> (!) z i = oR i"
     by (simp add: z_def Z_def SR_sub_read0 read0_sub_may)
 
   have Good_normalize_R:
     "Good as s ((!) ?x) ((!) z) = Good as s ((!) ?x) oR"
   proof -
     have Rwin_eq:
-      "⋀j. j < length (enumR as s kk) ⟹
+      "\<And>j. j < length (enumR as s kk) \<Longrightarrow>
            Rval_at as s ((!) z) j = Rval_at as s oR j"
     proof -
       fix j assume jR: "j < length (enumR as s kk)"
@@ -2059,8 +2190,8 @@ proof -
         fix t assume tlt: "t < length (map ((!) z) [?a..< ?a+?w])"
         hence tw: "t < ?w" by simp
         have idx: "[?a..< ?a+?w] ! t = ?a + t" using tw by simp
-        have mem: "?a + t ∈ blockR_abs enc0 as s kk j" by (simp add: blk tw)
-        have in_may: "?a + t ∈ may_read"
+        have mem: "?a + t \<in> blockR_abs enc0 as s kk j" by (simp add: blk tw)
+        have in_may: "?a + t \<in> may_read"
           unfolding may_read_def
           by (intro UnI2) (simp add: Rset_def blockR_abs_def UN_iff jR)
         show "map ((!) z) [?a..< ?a+?w] ! t = map oR [?a..< ?a+?w] ! t"
@@ -2076,9 +2207,9 @@ proof -
   have run_xz_eq_xoR:
     "run ((!) ?x) ((!) z) ?T = run ((!) ?x) oR ?T"
   proof (rule run_agrees_on_seen)
-    show "⋀i. i ∈ seenL_run ((!) ?x) ((!) z) ?T ⟹ (!) ?x i = (!) ?x i" by simp
+    show "\<And>i. i \<in> seenL_run ((!) ?x) ((!) z) ?T \<Longrightarrow> (!) ?x i = (!) ?x i" by simp
   next
-    show "⋀i. i ∈ seenR_run ((!) ?x) ((!) z) ?T ⟹ (!) z i = oR i"
+    show "\<And>i. i \<in> seenR_run ((!) ?x) ((!) z) ?T \<Longrightarrow> (!) z i = oR i"
       by (rule agree_on_seenR)
   qed
 
@@ -2087,20 +2218,20 @@ proof -
     by (rule correct_T0)
 
   have SR_sub_read0_x:
-    "seenR_run ((!) ?x) ((!) ?x) ?T ⊆ Base.read0 M ?x"
+    "seenR_run ((!) ?x) ((!) ?x) ?T \<subseteq> Base.read0 M ?x"
     by (rule seenR_T0_subset_read0) simp
 
   have run_xz_eq_xx:
     "run ((!) ?x) ((!) z) ?T = run ((!) ?x) ((!) ?x) ?T"
   proof (rule run_agrees_on_seen)
-    show "⋀i. i ∈ seenL_run ((!) ?x) ((!) z) ?T ⟹ (!) ?x i = (!) ?x i" 
+    show "\<And>i. i \<in> seenL_run ((!) ?x) ((!) z) ?T \<Longrightarrow> (!) ?x i = (!) ?x i" 
       by simp
   next
-    show "⋀i. i ∈ seenR_run ((!) ?x) ((!) z) ?T ⟹ (!) z i = (!) ?x i"
+    show "\<And>i. i \<in> seenR_run ((!) ?x) ((!) z) ?T \<Longrightarrow> (!) z i = (!) ?x i"
     proof -
-      fix i assume iSR: "i ∈ seenR_run ((!) ?x) ((!) z) ?T"
-      from SR_sub_read0 iSR have "i ∈ Base.read0 M ?x" by blast
-      with read0_sub_may have "i ∈ may_read" by blast
+      fix i assume iSR: "i \<in> seenR_run ((!) ?x) ((!) z) ?T"
+      from SR_sub_read0 iSR have "i \<in> Base.read0 M ?x" by blast
+      with read0_sub_may have "i \<in> may_read" by blast
       thus "(!) z i = (!) ?x i" by (simp add: z_def Z_def)
     qed
   qed
@@ -2128,12 +2259,12 @@ lemma run_T0_left_bridge:
 
 lemma run_T0_encR_catalog:
   "run oL ((!) (x0 as s)) (T0 as s)
-   = (∃jL<length (enumL as s kk). Lval_at as s oL jL ∈ set (enumR as s kk))"
+   = (\<exists>jL<length (enumL as s kk). Lval_at as s oL jL \<in> set (enumR as s kk))"
   by (simp add: run_T0_mixed_bridge Good_char_encR)
 
 lemma run_T0_encL_catalog:
   "run ((!) (x0 as s)) oR (T0 as s)
-   = (∃jR<length (enumR as s kk). Rval_at as s oR jR ∈ set (enumL as s kk))"
+   = (\<exists>jR<length (enumR as s kk). Rval_at as s oR jR \<in> set (enumL as s kk))"
   by (simp add: run_T0_left_bridge Good_char_encL)
 
 (* 3) Mixed bridge: run on T0 with (oL, encR) equals Good with (oL, encR) *)
@@ -2145,15 +2276,15 @@ lemma Lval_at_on_x0_block[simp]:
 
 lemma flipR_setval:
   assumes jR: "j < length (enumR as s kk)"
-      and R2: "2 ≤ length (enumR as s kk)"
-      and vR: "v ∈ set (enumR as s kk)"
+      and R2: "2 \<le> length (enumR as s kk)"
+      and vR: "v \<in> set (enumR as s kk)"
   shows
-    "∃oR'. (∀i. i ∉ blockR_abs enc0 as s kk j ⟶ oR' i = (x0 as s) ! i)
-         ∧  Rval_at as s oR' j = v"
+    "\<exists>oR'. (\<forall>i. i \<notin> blockR_abs enc0 as s kk j \<longrightarrow> oR' i = (x0 as s) ! i)
+         \<and>  Rval_at as s oR' j = v"
 proof -
   define a where "a = length (enc0 as s) + offR as s kk j"
   define w where "w = W as s"
-  have BND: "a + w ≤ length (x0 as s)"
+  have BND: "a + w \<le> length (x0 as s)"
     by (simp add: a_def w_def offR_window_in_enc[OF jR])
 
   (* choose the fixed-width bit pattern for v *)
@@ -2162,10 +2293,10 @@ proof -
 
   (* build oR' by overwriting exactly the j-th R block with pat *)
   define oR' where
-    "oR' i = (if i ∈ {a ..< a + w} then pat ! (i - a) else (x0 as s) ! i)" for i
+    "oR' i = (if i \<in> {a ..< a + w} then pat ! (i - a) else (x0 as s) ! i)" for i
 
   have outside:
-    "∀i. i ∉ blockR_abs enc0 as s kk j ⟶ oR' i = (x0 as s) ! i"
+    "\<forall>i. i \<notin> blockR_abs enc0 as s kk j \<longrightarrow> oR' i = (x0 as s) ! i"
     by (simp add: oR'_def a_def w_def blockR_abs_def offR_def)
 
   (* slice [a ..< a+w] equals pat under oR' *)
@@ -2176,7 +2307,7 @@ proof -
     fix t assume "t < length (map oR' [a ..< a + w])"
     hence tw: "t < w" by simp
     have idx: "[a ..< a + w] ! t = a + t" using tw by simp
-    have inblk: "a ≤ a + t ∧ a + t < a + w" using tw by simp
+    have inblk: "a \<le> a + t \<and> a + t < a + w" using tw by simp
     show "map oR' [a ..< a + w] ! t = pat ! t"
       using nth_map idx oR'_def inblk by (simp add: tw)
   qed
@@ -2197,26 +2328,26 @@ qed
 
 lemma Run_unread_R:
   fixes x y :: "bool list"
-  assumes DISJ:  "Base.read0 M x ∩ blockR_abs enc0 as s kk j = {}"
-  assumes AGREE: "⋀i. i ∉ blockR_abs enc0 as s kk j ⟹ y ! i = x ! i"
+  assumes DISJ:  "Base.read0 M x \<inter> blockR_abs enc0 as s kk j = {}"
+  assumes AGREE: "\<And>i. i \<notin> blockR_abs enc0 as s kk j \<Longrightarrow> y ! i = x ! i"
   assumes X:     "x = enc as s kk"
   shows "run ((!) x) ((!) y) (T0 as s) = run ((!) x) ((!) x) (T0 as s)"
 proof -
-  have SRsub: "seenR_run ((!) x) ((!) y) (T0 as s) ⊆ Base.read0 M x"
+  have SRsub: "seenR_run ((!) x) ((!) y) (T0 as s) \<subseteq> Base.read0 M x"
     by (rule seenR_T0_subset_read0[OF X])
   have agree_on_seenR:
-    "⋀i. i ∈ seenR_run ((!) x) ((!) y) (T0 as s) ⟹ (!) y i = (!) x i"
+    "\<And>i. i \<in> seenR_run ((!) x) ((!) y) (T0 as s) \<Longrightarrow> (!) y i = (!) x i"
   proof -
-    fix i assume "i ∈ seenR_run ((!) x) ((!) y) (T0 as s)"
-    with SRsub have "i ∈ Base.read0 M x" by blast
-    with DISJ have "i ∉ blockR_abs enc0 as s kk j" by auto
+    fix i assume "i \<in> seenR_run ((!) x) ((!) y) (T0 as s)"
+    with SRsub have "i \<in> Base.read0 M x" by blast
+    with DISJ have "i \<notin> blockR_abs enc0 as s kk j" by auto
     with AGREE show "(!) y i = (!) x i" by simp
   qed
   show ?thesis
   proof (rule run_agrees_on_seen)
-    show "⋀i. i ∈ seenL_run ((!) x) ((!) y) (T0 as s) ⟹ (!) x i = (!) x i" by simp
+    show "\<And>i. i \<in> seenL_run ((!) x) ((!) y) (T0 as s) \<Longrightarrow> (!) x i = (!) x i" by simp
   next
-    show "⋀i. i ∈ seenR_run ((!) x) ((!) y) (T0 as s) ⟹ (!) y i = (!) x i"
+    show "\<And>i. i \<in> seenR_run ((!) x) ((!) y) (T0 as s) \<Longrightarrow> (!) y i = (!) x i"
       by (rule agree_on_seenR)
   qed
 qed
@@ -2224,8 +2355,8 @@ qed
 lemma blockR_pairwise_disjoint:
   assumes jR:  "j  < length (enumR as s kk)"
       and j'R: "j' < length (enumR as s kk)"
-      and ne:  "j ≠ j'"
-  shows "blockR_abs enc0 as s kk j ∩ blockR_abs enc0 as s kk j' = {}"
+      and ne:  "j \<noteq> j'"
+  shows "blockR_abs enc0 as s kk j \<inter> blockR_abs enc0 as s kk j' = {}"
   using ne
   by (rule blockR_abs_disjoint)
 
@@ -2233,8 +2364,8 @@ lemma x0_is_enc[simp]: "x0 as s = enc as s kk"
   by simp
 
 lemma Good_unread_L_local:
-  assumes disj: "Base.read0 M x ∩ blockL_abs enc0 as s j = {}"
-  assumes out:  "⋀i. i ∉ blockL_abs enc0 as s j ⟹ y ! i = x ! i"
+  assumes disj: "Base.read0 M x \<inter> blockL_abs enc0 as s j = {}"
+  assumes out:  "\<And>i. i \<notin> blockL_abs enc0 as s j \<Longrightarrow> y ! i = x ! i"
   assumes X:    "x = enc as s kk"
   shows "Good as s ((!) y) ((!) x) = Good as s ((!) x) ((!) x)"
 proof -
@@ -2243,16 +2374,16 @@ proof -
 
   (* T0’s left-seen set is contained in read0 on x0-inputs *)
   have SLsub:
-    "seenL_run ((!) y) ((!) x) (T0 as s) ⊆ Base.read0 M x"
+    "seenL_run ((!) y) ((!) x) (T0 as s) \<subseteq> Base.read0 M x"
     by (rule seenL_T0_subset_read0[OF X0])
 
   (* y and x agree on everything T0 ever looks at on the left *)
   have agree_on_seenL:
-    "⋀i. i ∈ seenL_run ((!) y) ((!) x) (T0 as s) ⟹ (!) y i = (!) x i"
+    "\<And>i. i \<in> seenL_run ((!) y) ((!) x) (T0 as s) \<Longrightarrow> (!) y i = (!) x i"
   proof -
-    fix i assume "i ∈ seenL_run ((!) y) ((!) x) (T0 as s)"
-    with SLsub have "i ∈ Base.read0 M x" by blast
-    with disj have "i ∉ blockL_abs enc0 as s j" by auto
+    fix i assume "i \<in> seenL_run ((!) y) ((!) x) (T0 as s)"
+    with SLsub have "i \<in> Base.read0 M x" by blast
+    with disj have "i \<notin> blockL_abs enc0 as s j" by auto
     with out show "(!) y i = (!) x i" by simp
   qed
 
@@ -2261,7 +2392,7 @@ proof -
     "run ((!) y) ((!) x) (T0 as s) = run ((!) x) ((!) x) (T0 as s)"
     by (rule run_agrees_on_seen) (simp_all add: agree_on_seenL)
 
-  (* bridge Good ↔ run: do it in two tiny steps to avoid purple *)
+  (* bridge Good \<leftrightarrow> run: do it in two tiny steps to avoid purple *)
   have G_yx_to_run0:
     "Good as s ((!) y) ((!) (x0 as s)) = run ((!) y) ((!) (x0 as s)) (T0 as s)"
     by (simp add: run_T0_mixed_bridge[symmetric])
@@ -2281,22 +2412,22 @@ proof -
 qed
 
 lemma coverage_for_enc_blocks_L:
-  assumes L2:   "2 ≤ length (enumL as s kk)"
-      and hit:  "∃v∈set (enumL as s kk). v ∈ set (enumR as s kk)"
-      and miss: "∃v∈set (enumL as s kk). v ∉ set (enumR as s kk)"
+  assumes L2:   "2 \<le> length (enumL as s kk)"
+      and hit:  "\<exists>v\<in>set (enumL as s kk). v \<in> set (enumR as s kk)"
+      and miss: "\<exists>v\<in>set (enumL as s kk). v \<notin> set (enumR as s kk)"
       and baseline_only_j:
-        "⋀j. Good as s ((!) (x0 as s)) ((!) (x0 as s)) ⟹
-             (∀j'<length (enumL as s kk). j' ≠ j ⟶
-                Lval_at as s ((!) (x0 as s)) j' ∉ set (enumR as s kk))"
-  shows "∀j<length (enumL as s kk). touches (x0 as s) (blockL_abs enc0 as s j)"
+        "\<And>j. Good as s ((!) (x0 as s)) ((!) (x0 as s)) \<Longrightarrow>
+             (\<forall>j'<length (enumL as s kk). j' \<noteq> j \<longrightarrow>
+                Lval_at as s ((!) (x0 as s)) j' \<notin> set (enumR as s kk))"
+  shows "\<forall>j<length (enumL as s kk). touches (x0 as s) (blockL_abs enc0 as s j)"
 proof (intro allI impI)
   fix j assume jL: "j < length (enumL as s kk)"
   let ?x = "x0 as s"
   show "touches ?x (blockL_abs enc0 as s j)"
   proof (rule ccontr)
-    assume NT: "¬ touches ?x (blockL_abs enc0 as s j)"
+    assume NT: "\<not> touches ?x (blockL_abs enc0 as s j)"
     then have not_touch:
-      "Base.read0 M ?x ∩ blockL_abs enc0 as s j = {}"
+      "Base.read0 M ?x \<inter> blockL_abs enc0 as s j = {}"
       by (simp add: touches_def)
 
     define a where "a = length (enc0 as s) + offL as s j"
@@ -2307,24 +2438,24 @@ proof (intro allI impI)
     have X0: "?x = enc as s kk" by simp
 
     consider (G) "Good as s ((!) ?x) ((!) ?x)"
-           | (NG) "¬ Good as s ((!) ?x) ((!) ?x)" by blast
+           | (NG) "\<not> Good as s ((!) ?x) ((!) ?x)" by blast
     then show False
     proof cases
       case G
-      from miss obtain v_out where vL: "v_out ∈ set (enumL as s kk)"
-                               and vNR: "v_out ∉ set (enumR as s kk)" by blast
+      from miss obtain v_out where vL: "v_out \<in> set (enumL as s kk)"
+                               and vNR: "v_out \<notin> set (enumR as s kk)" by blast
       obtain pat where pat_len: "length pat = w" and pat_val: "from_bits pat = v_out"
         using vL bits_roundtrip w_def by blast
-      define oL' where "oL' i = (if i ∈ {a..<a + w} then pat ! (i - a) else ?x ! i)" for i
+      define oL' where "oL' i = (if i \<in> {a..<a + w} then pat ! (i - a) else ?x ! i)" for i
       define y where "y = splice a w ?x (map oL' [a..<a + w])"
 
       have LEN: "length (map oL' [a..<a + w]) = w" by simp
       have outside_y:
-        "⋀i. i ∉ blockL_abs enc0 as s j ⟹ y ! i = ?x ! i"
+        "\<And>i. i \<notin> blockL_abs enc0 as s j \<Longrightarrow> y ! i = ?x ! i"
       proof -
-        fix i assume nin: "i ∉ blockL_abs enc0 as s j"
-        with blk_repr have nin': "i ∉ {a..<a + w}" by simp
-        have AL: "a ≤ length ?x" using offL_window_in_enc[OF jL] a_def w_def by linarith
+        fix i assume nin: "i \<notin> blockL_abs enc0 as s j"
+        with blk_repr have nin': "i \<notin> {a..<a + w}" by simp
+        have AL: "a \<le> length ?x" using offL_window_in_enc[OF jL] a_def w_def by linarith
         show "y ! i = ?x ! i"
           using nin' by (cases "i < a")
                         (simp_all add: y_def splice_nth_left AL splice_nth_right[OF LEN])
@@ -2345,15 +2476,15 @@ proof (intro allI impI)
         unfolding Lval_at_def a_def w_def
         by (simp add: slice_pat from_bits.simps)
 
-      have Good_y: "¬ Good as s ((!) y) ((!) ?x)"
+      have Good_y: "\<not> Good as s ((!) y) ((!) ?x)"
       proof -
-        have "Lval_at as s ((!) y) j ∉ set (enumR as s kk)"
+        have "Lval_at as s ((!) y) j \<notin> set (enumR as s kk)"
           using Lj_y vNR by simp
         moreover have
-          "⋀j'. j' < length (enumL as s kk) ⟹ j' ≠ j ⟹
-             Lval_at as s ((!) y) j' ∉ set (enumR as s kk)"
+          "\<And>j'. j' < length (enumL as s kk) \<Longrightarrow> j' \<noteq> j \<Longrightarrow>
+             Lval_at as s ((!) y) j' \<notin> set (enumR as s kk)"
         proof -
-          fix j' assume j'lt: "j' < length (enumL as s kk)" and ne: "j' ≠ j"
+          fix j' assume j'lt: "j' < length (enumL as s kk)" and ne: "j' \<noteq> j"
           have eq_other:
             "Lval_at as s ((!) y) j' = Lval_at as s ((!) ?x) j'"
           proof -
@@ -2361,9 +2492,9 @@ proof (intro allI impI)
             define w' where "w' = W as s"
             have blk': "blockL_abs enc0 as s j' = {a'..<a'+w'}"
               by (simp add: a'_def w'_def blockL_abs_def offL_def)
-            have disj: "blockL_abs enc0 as s j ∩ blockL_abs enc0 as s j' = {}"
+            have disj: "blockL_abs enc0 as s j \<inter> blockL_abs enc0 as s j' = {}"
               using blockL_abs_disjoint[OF ne].
-            have eq_on: "⋀i. i ∈ blockL_abs enc0 as s j' ⟹ y ! i = ?x ! i"
+            have eq_on: "\<And>i. i \<in> blockL_abs enc0 as s j' \<Longrightarrow> y ! i = ?x ! i"
               using outside_y by (intro) (use disj in auto)
             show ?thesis
             proof (rule nth_equalityI)
@@ -2373,14 +2504,14 @@ proof (intro allI impI)
               fix t assume tlt: "t < length (map ((!) y) [a'..<a'+w'])"
               hence tw: "t < w'" by simp
               have idx: "[a'..<a'+w'] ! t = a' + t" using tw by simp
-              have mem: "a' + t ∈ blockL_abs enc0 as s j'" by (simp add: blk' tw)
+              have mem: "a' + t \<in> blockL_abs enc0 as s j'" by (simp add: blk' tw)
               show "map ((!) y) [a'..<a'+w'] ! t
                     = map ((!) ?x) [a'..<a'+w'] ! t"
                 by (simp add: idx tw eq_on[OF mem])
             qed
           qed
           from baseline_only_j[OF G, of j'] j'lt ne show
-            "Lval_at as s ((!) y) j' ∉ set (enumR as s kk)"
+            "Lval_at as s ((!) y) j' \<notin> set (enumR as s kk)"
             by (simp add: eq_other)
         qed
         ultimately show ?thesis
@@ -2395,20 +2526,20 @@ proof (intro allI impI)
 
     next
       case NG
-      from hit obtain v_in where vL: "v_in ∈ set (enumL as s kk)"
-                             and vR: "v_in ∈ set (enumR as s kk)" by blast
+      from hit obtain v_in where vL: "v_in \<in> set (enumL as s kk)"
+                             and vR: "v_in \<in> set (enumR as s kk)" by blast
       obtain pat where pat_len: "length pat = w" and pat_val: "from_bits pat = v_in"
         using vL bits_roundtrip w_def by blast
-      define oL' where "oL' i = (if i ∈ {a..<a + w} then pat ! (i - a) else ?x ! i)" for i
+      define oL' where "oL' i = (if i \<in> {a..<a + w} then pat ! (i - a) else ?x ! i)" for i
       define y where "y = splice a w ?x (map oL' [a..<a + w])"
 
       have LEN: "length (map oL' [a..<a + w]) = w" by simp
       have outside_y:
-        "⋀i. i ∉ blockL_abs enc0 as s j ⟹ y ! i = ?x ! i"
+        "\<And>i. i \<notin> blockL_abs enc0 as s j \<Longrightarrow> y ! i = ?x ! i"
       proof -
-        fix i assume nin: "i ∉ blockL_abs enc0 as s j"
-        with blk_repr have nin': "i ∉ {a..<a + w}" by simp
-        have AL: "a ≤ length ?x" using offL_window_in_enc[OF jL] a_def w_def by linarith
+        fix i assume nin: "i \<notin> blockL_abs enc0 as s j"
+        with blk_repr have nin': "i \<notin> {a..<a + w}" by simp
+        have AL: "a \<le> length ?x" using offL_window_in_enc[OF jL] a_def w_def by linarith
         show "y ! i = ?x ! i"
           using nin' by (cases "i < a")
                         (simp_all add: y_def splice_nth_left AL splice_nth_right[OF LEN])
@@ -2431,10 +2562,10 @@ proof (intro allI impI)
 
       have Good_y: "Good as s ((!) y) ((!) ?x)"
       proof -
-        have "Lval_at as s ((!) y) j ∈ set (enumR as s kk)"
+        have "Lval_at as s ((!) y) j \<in> set (enumR as s kk)"
           using Lj_y vR by simp
-        hence "∃jL<length (enumL as s kk).
-                 Lval_at as s ((!) y) jL ∈ set (enumR as s kk)"
+        hence "\<exists>jL<length (enumL as s kk).
+                 Lval_at as s ((!) y) jL \<in> set (enumR as s kk)"
           using jL by blast
         thus ?thesis
           by (simp add: Good_char_encR)
@@ -2450,8 +2581,8 @@ proof (intro allI impI)
 qed
 
 lemma Good_unread_R_local:
-  assumes disj: "Base.read0 M x ∩ blockR_abs enc0 as s kk j = {}"
-  assumes out:  "⋀i. i ∉ blockR_abs enc0 as s kk j ⟹ y ! i = x ! i"
+  assumes disj: "Base.read0 M x \<inter> blockR_abs enc0 as s kk j = {}"
+  assumes out:  "\<And>i. i \<notin> blockR_abs enc0 as s kk j \<Longrightarrow> y ! i = x ! i"
   assumes X:    "x = enc as s kk"
   shows "Good as s ((!) x) ((!) y) = Good as s ((!) x) ((!) x)"
 proof -
@@ -2474,28 +2605,28 @@ proof -
 qed
 
 lemma coverage_for_enc_blocks_R:
-  assumes R2:  "2 ≤ length (enumR as s kk)"
-      and hitR:  "∃v∈set (enumR as s kk). v ∈ set (enumL as s kk)"
-      and missR: "∃v∈set (enumR as s kk). v ∉ set (enumL as s kk)"
+  assumes R2:  "2 \<le> length (enumR as s kk)"
+      and hitR:  "\<exists>v\<in>set (enumR as s kk). v \<in> set (enumL as s kk)"
+      and missR: "\<exists>v\<in>set (enumR as s kk). v \<notin> set (enumL as s kk)"
       and baseline_only_jR:
-        "⋀j. Good as s ((!) (x0 as s)) ((!) (x0 as s)) ⟹
-             (∀j'<length (enumR as s kk). j' ≠ j ⟶
-                Rval_at as s ((!) (x0 as s)) j' ∉ set (enumL as s kk))"
-  shows "∀j<length (enumR as s kk). touches (x0 as s) (blockR_abs enc0 as s kk j)"
+        "\<And>j. Good as s ((!) (x0 as s)) ((!) (x0 as s)) \<Longrightarrow>
+             (\<forall>j'<length (enumR as s kk). j' \<noteq> j \<longrightarrow>
+                Rval_at as s ((!) (x0 as s)) j' \<notin> set (enumL as s kk))"
+  shows "\<forall>j<length (enumR as s kk). touches (x0 as s) (blockR_abs enc0 as s kk j)"
 proof (intro allI impI)
   fix j assume jR: "j < length (enumR as s kk)"
   let ?x = "x0 as s"
 
   show "touches ?x (blockR_abs enc0 as s kk j)"
   proof (rule ccontr)
-    assume NT: "¬ touches ?x (blockR_abs enc0 as s kk j)"
+    assume NT: "\<not> touches ?x (blockR_abs enc0 as s kk j)"
     then have not_touch:
-      "Base.read0 M ?x ∩ blockR_abs enc0 as s kk j = {}"
+      "Base.read0 M ?x \<inter> blockR_abs enc0 as s kk j = {}"
       by (simp add: touches_def)
 
     define a where "a = length (enc0 as s) + offR as s kk j"
     define w where "w = W as s"
-    have BND: "a + w ≤ length ?x"
+    have BND: "a + w \<le> length ?x"
       by (simp add: a_def w_def offR_window_in_enc[OF jR])
     have blk_repr: "blockR_abs enc0 as s kk j = {a..<a + w}"
       by (simp add: a_def w_def blockR_abs_def offR_def length_padL)
@@ -2503,24 +2634,24 @@ proof (intro allI impI)
     have X0: "?x = enc as s kk" by simp
 
     consider (G) "Good as s ((!) ?x) ((!) ?x)"
-           | (NG) "¬ Good as s ((!) ?x) ((!) ?x)" by blast
+           | (NG) "\<not> Good as s ((!) ?x) ((!) ?x)" by blast
     then show False
     proof cases
       case G
-      from missR obtain v_out where vR: "v_out ∈ set (enumR as s kk)"
-                               and vNL: "v_out ∉ set (enumL as s kk)" by blast
+      from missR obtain v_out where vR: "v_out \<in> set (enumR as s kk)"
+                               and vNL: "v_out \<notin> set (enumL as s kk)" by blast
       obtain pat where pat_len: "length pat = w" and pat_val: "from_bits pat = v_out"
         using vR bits_roundtrip w_def by blast
-      define oR' where "oR' i = (if i ∈ {a..<a + w} then pat ! (i - a) else ?x ! i)" for i
+      define oR' where "oR' i = (if i \<in> {a..<a + w} then pat ! (i - a) else ?x ! i)" for i
       have LEN: "length (map oR' [a..<a + w]) = w" by simp
       define y where "y = splice a w ?x (map oR' [a..<a + w])"
 
       have outside_y:
-        "⋀i. i ∉ blockR_abs enc0 as s kk j ⟹ y ! i = ?x ! i"
+        "\<And>i. i \<notin> blockR_abs enc0 as s kk j \<Longrightarrow> y ! i = ?x ! i"
       proof -
-        fix i assume nin: "i ∉ blockR_abs enc0 as s kk j"
-        with blk_repr have nin': "i ∉ {a..<a + w}" by simp
-        have AL: "a ≤ length ?x" using BND by linarith
+        fix i assume nin: "i \<notin> blockR_abs enc0 as s kk j"
+        with blk_repr have nin': "i \<notin> {a..<a + w}" by simp
+        have AL: "a \<le> length ?x" using BND by linarith
         show "y ! i = ?x ! i"
           using nin'
           by (cases "i < a")
@@ -2538,10 +2669,10 @@ proof (intro allI impI)
           by (simp add: oR'_def idx tw)
       qed
 
-      have inside_y: "⋀i. i ∈ {a..<a + w} ⟹ y ! i = oR' i"
+      have inside_y: "\<And>i. i \<in> {a..<a + w} \<Longrightarrow> y ! i = oR' i"
       proof -
-        fix i assume "i ∈ {a..<a + w}"
-        then have ai: "a ≤ i" and ilt: "i < a + w" by auto
+        fix i assume "i \<in> {a..<a + w}"
+        then have ai: "a \<le> i" and ilt: "i < a + w" by auto
         have "y ! i = (map oR' [a..<a + w]) ! (i - a)"
           by (simp add: y_def splice_nth_inside[OF LEN BND ai ilt])
         also have "... = oR' i" using ai ilt by force
@@ -2565,18 +2696,18 @@ proof (intro allI impI)
       qed
 
       have same_others:
-        "⋀j'. j' < length (enumR as s kk) ⟹ j' ≠ j ⟹
+        "\<And>j'. j' < length (enumR as s kk) \<Longrightarrow> j' \<noteq> j \<Longrightarrow>
               Rval_at as s ((!) y) j' = Rval_at as s ((!) ?x) j'"
       proof -
-        fix j' assume j'R: "j' < length (enumR as s kk)" and ne: "j' ≠ j"
+        fix j' assume j'R: "j' < length (enumR as s kk)" and ne: "j' \<noteq> j"
         define a' where "a' = length (enc0 as s) + offR as s kk j'"
         define w' where "w' = W as s"
         have blk': "blockR_abs enc0 as s kk j' = {a'..<a' + w'}"
           by (simp add: a'_def w'_def blockR_abs_def offR_def length_padL)
         have disj0:
-          "blockR_abs enc0 as s kk j' ∩ blockR_abs enc0 as s kk j = {}"
+          "blockR_abs enc0 as s kk j' \<inter> blockR_abs enc0 as s kk j = {}"
           by (rule blockR_pairwise_disjoint[OF j'R jR ne])
-        have eq_on: "⋀i. i ∈ blockR_abs enc0 as s kk j' ⟹ y ! i = ?x ! i"
+        have eq_on: "\<And>i. i \<in> blockR_abs enc0 as s kk j' \<Longrightarrow> y ! i = ?x ! i"
           using IntI disj0 outside_y by fastforce
         have "map ((!) y) [a'..<a' + w'] = map ((!) ?x) [a'..<a' + w']"
         proof (rule nth_equalityI)
@@ -2586,7 +2717,7 @@ proof (intro allI impI)
           fix t assume "t < length (map ((!) y) [a'..<a' + w'])"
           then have tw: "t < w'" by simp
           have idx: "[a'..<a' + w'] ! t = a' + t" using tw by simp
-          have mem: "a' + t ∈ blockR_abs enc0 as s kk j'"
+          have mem: "a' + t \<in> blockR_abs enc0 as s kk j'"
             by (simp add: blk' tw)
           show "map ((!) y) [a'..<a' + w'] ! t
               = map ((!) ?x) [a'..<a' + w'] ! t"
@@ -2597,16 +2728,16 @@ proof (intro allI impI)
       qed
 
       have not_good_y:
-        "¬ Good as s ((!) ?x) ((!) y)"
+        "\<not> Good as s ((!) ?x) ((!) y)"
       proof -
         have others:
-          "⋀j'. j' < length (enumR as s kk) ⟹ j' ≠ j ⟹
-              Rval_at as s ((!) y) j' ∉ set (enumL as s kk)"
+          "\<And>j'. j' < length (enumR as s kk) \<Longrightarrow> j' \<noteq> j \<Longrightarrow>
+              Rval_at as s ((!) y) j' \<notin> set (enumL as s kk)"
           using baseline_only_jR[OF G] same_others by auto
-        have "Rval_at as s ((!) y) j ∉ set (enumL as s kk)"
+        have "Rval_at as s ((!) y) j \<notin> set (enumL as s kk)"
           using Rj_y vNL by simp
-        hence "¬ (∃jR<length (enumR as s kk).
-                     Rval_at as s ((!) y) jR ∈ set (enumL as s kk))"
+        hence "\<not> (\<exists>jR<length (enumR as s kk).
+                     Rval_at as s ((!) y) jR \<in> set (enumL as s kk))"
           using others jR by auto
         thus ?thesis using Good_char_encL by blast
       qed
@@ -2619,20 +2750,20 @@ proof (intro allI impI)
 
     next
       case NG
-      from hitR obtain v_in where vR: "v_in ∈ set (enumR as s kk)"
-                               and vL: "v_in ∈ set (enumL as s kk)" by blast
+      from hitR obtain v_in where vR: "v_in \<in> set (enumR as s kk)"
+                               and vL: "v_in \<in> set (enumL as s kk)" by blast
       obtain pat where pat_len: "length pat = w" and pat_val: "from_bits pat = v_in"
         using vR bits_roundtrip w_def by blast
-      define oR' where "oR' i = (if i ∈ {a..<a + w} then pat ! (i - a) else ?x ! i)" for i
+      define oR' where "oR' i = (if i \<in> {a..<a + w} then pat ! (i - a) else ?x ! i)" for i
       have LEN: "length (map oR' [a..<a + w]) = w" by simp
       define y where "y = splice a w ?x (map oR' [a..<a + w])"
 
       have outside_y:
-        "⋀i. i ∉ blockR_abs enc0 as s kk j ⟹ y ! i = ?x ! i"
+        "\<And>i. i \<notin> blockR_abs enc0 as s kk j \<Longrightarrow> y ! i = ?x ! i"
       proof -
-        fix i assume nin: "i ∉ blockR_abs enc0 as s kk j"
-        with blk_repr have nin': "i ∉ {a..<a + w}" by simp
-        have AL: "a ≤ length ?x" using BND by linarith
+        fix i assume nin: "i \<notin> blockR_abs enc0 as s kk j"
+        with blk_repr have nin': "i \<notin> {a..<a + w}" by simp
+        have AL: "a \<le> length ?x" using BND by linarith
         show "y ! i = ?x ! i"
           using nin'
           by (cases "i < a")
@@ -2650,10 +2781,10 @@ proof (intro allI impI)
           by (simp add: oR'_def idx tw)
       qed
 
-      have inside: "⋀i. i ∈ {a..<a + w} ⟹ y ! i = oR' i"
+      have inside: "\<And>i. i \<in> {a..<a + w} \<Longrightarrow> y ! i = oR' i"
       proof -
-        fix i assume iB: "i ∈ {a..<a + w}"
-        then have ai: "a ≤ i" and ilt: "i < a + w" by auto
+        fix i assume iB: "i \<in> {a..<a + w}"
+        then have ai: "a \<le> i" and ilt: "i < a + w" by auto
         have "y ! i = (map oR' [a..<a + w]) ! (i - a)"
           by (simp add: y_def splice_nth_inside[OF LEN BND ai ilt])
         also have "... = oR' i" using ai ilt by force
@@ -2677,10 +2808,10 @@ proof (intro allI impI)
 
       have Good_y: "Good as s ((!) ?x) ((!) y)"
       proof -
-        have "Rval_at as s ((!) y) j ∈ set (enumL as s kk)"
+        have "Rval_at as s ((!) y) j \<in> set (enumL as s kk)"
           using Rj_y vL by simp
-        hence "∃jR<length (enumR as s kk).
-                 Rval_at as s ((!) y) jR ∈ set (enumL as s kk)"
+        hence "\<exists>jR<length (enumR as s kk).
+                 Rval_at as s ((!) y) jR \<in> set (enumL as s kk)"
           using jR by blast
         thus ?thesis by (simp add: Good_char_encL)
       qed
@@ -2700,60 +2831,60 @@ qed
 
 lemma coverage_blocks:
   assumes "n = length as" "distinct_subset_sums as"
-      and L2:   "2 ≤ length (enumL as s kk)"
-      and hitL: "∃v∈set (enumL as s kk). v ∈ set (enumR as s kk)"
-      and missL:"∃v∈set (enumL as s kk). v ∉ set (enumR as s kk)"
+      and L2:   "2 \<le> length (enumL as s kk)"
+      and hitL: "\<exists>v\<in>set (enumL as s kk). v \<in> set (enumR as s kk)"
+      and missL:"\<exists>v\<in>set (enumL as s kk). v \<notin> set (enumR as s kk)"
       and base_only_L:
-           "⋀j. Good as s ((!) (enc as s kk)) ((!) (enc as s kk)) ⟶
-                (∀j'<length (enumL as s kk). j' ≠ j ⟶
-                   Lval_at as s ((!) (enc as s kk)) j' ∉ set (enumR as s kk))"
-      and R2:   "2 ≤ length (enumR as s kk)"
-      and hitR: "∃v∈set (enumR as s kk). v ∈ set (enumL as s kk)"
-      and missR:"∃v∈set (enumR as s kk). v ∉ set (enumL as s kk)"
+           "\<And>j. Good as s ((!) (enc as s kk)) ((!) (enc as s kk)) \<longrightarrow>
+                (\<forall>j'<length (enumL as s kk). j' \<noteq> j \<longrightarrow>
+                   Lval_at as s ((!) (enc as s kk)) j' \<notin> set (enumR as s kk))"
+      and R2:   "2 \<le> length (enumR as s kk)"
+      and hitR: "\<exists>v\<in>set (enumR as s kk). v \<in> set (enumL as s kk)"
+      and missR:"\<exists>v\<in>set (enumR as s kk). v \<notin> set (enumL as s kk)"
       and base_only_R:
-           "⋀j. Good as s ((!) (x0 as s)) ((!) (x0 as s)) ⟶
-                (∀j'<length (enumR as s kk). j' ≠ j ⟶
-                   Rval_at as s ((!) (x0 as s)) j' ∉ set (enumL as s kk))"
+           "\<And>j. Good as s ((!) (x0 as s)) ((!) (x0 as s)) \<longrightarrow>
+                (\<forall>j'<length (enumR as s kk). j' \<noteq> j \<longrightarrow>
+                   Rval_at as s ((!) (x0 as s)) j' \<notin> set (enumL as s kk))"
   shows
-   "(∀j<length (enumL as s kk). touches (enc as s kk) (blockL_abs enc0 as s j)) ∧
-    (∀j<length (enumR as s kk). touches (enc as s kk) (blockR_abs enc0 as s kk j))"
+   "(\<forall>j<length (enumL as s kk). touches (enc as s kk) (blockL_abs enc0 as s j)) \<and>
+    (\<forall>j<length (enumR as s kk). touches (enc as s kk) (blockR_abs enc0 as s kk j))"
 proof
-  show "∀j<length (enumL as s kk). touches (enc as s kk) (blockL_abs enc0 as s j)"
+  show "\<forall>j<length (enumL as s kk). touches (enc as s kk) (blockL_abs enc0 as s j)"
     using coverage_for_enc_blocks_L[OF L2 hitL missL base_only_L] .
 
   have base_only_R':
-  "⋀j. Good as s ((!) (x0 as s)) ((!) (x0 as s)) ⟹
-       (∀j'<length (enumR as s kk). j' ≠ j ⟶
-          Rval_at as s ((!) (x0 as s)) j' ∉ set (enumL as s kk))"
+  "\<And>j. Good as s ((!) (x0 as s)) ((!) (x0 as s)) \<Longrightarrow>
+       (\<forall>j'<length (enumR as s kk). j' \<noteq> j \<longrightarrow>
+          Rval_at as s ((!) (x0 as s)) j' \<notin> set (enumL as s kk))"
     using base_only_R by blast
 
   have Rcov:
-  "∀j<length (enumR as s kk). touches (x0 as s) (blockR_abs enc0 as s kk j)"
+  "\<forall>j<length (enumR as s kk). touches (x0 as s) (blockR_abs enc0 as s kk j)"
     using R2 hitR missR base_only_R'
   by (rule coverage_for_enc_blocks_R)
-  have "∀j<length (enumR as s kk). touches (enc as s kk) (blockR_abs enc0 as s kk j)"
+  have "\<forall>j<length (enumR as s kk). touches (enc as s kk) (blockR_abs enc0 as s kk j)"
     using Rcov by blast  (* relies on x0_is_enc[simp] *)
-  show "∀j<length (enumR as s kk). touches (enc as s kk) (blockR_abs enc0 as s kk j)"
+  show "\<forall>j<length (enumR as s kk). touches (enc as s kk) (blockR_abs enc0 as s kk j)"
     using Rcov by blast  (* uses x0_is_enc[simp] *)
 qed
 
 lemma steps_lower_bound_core:
-  assumes Lcov_ALL: "∀j<length (enumL as s kk). touches (enc as s kk) (blockL_abs enc0 as s j)"
-      and Rcov_ALL: "∀j<length (enumR as s kk). touches (enc as s kk) (blockR_abs enc0 as s kk j)"
+  assumes Lcov_ALL: "\<forall>j<length (enumL as s kk). touches (enc as s kk) (blockL_abs enc0 as s j)"
+      and Rcov_ALL: "\<forall>j<length (enumR as s kk). touches (enc as s kk) (blockR_abs enc0 as s kk j)"
       and n_def: "n = length as"
-  shows "steps M (enc as s kk) ≥
+  shows "steps M (enc as s kk) \<ge>
            card (LHS (e_k as s kk) n) + card (RHS (e_k as s kk) n)"
 proof -
-  (* After you derived the two “forall … touches …” facts: *)
+  (* After you derived the two “forall \<dots> touches \<dots>” facts: *)
   have Lcov_ALL:
-    "∀j<length (enumL as s kk). touches (x0 as s) (blockL_abs enc0 as s j)" by fact
+    "\<forall>j<length (enumL as s kk). touches (x0 as s) (blockL_abs enc0 as s j)" by fact
   have Rcov_ALL:
-    "∀j<length (enumR as s kk). touches (x0 as s) (blockR_abs enc0 as s kk j)" by fact
+    "\<forall>j<length (enumR as s kk). touches (x0 as s) (blockR_abs enc0 as s kk j)" by fact
 
  (* Turn them into pointwise rules you can use later *)
-  have Lcov: "⋀j. j < length (enumL as s kk) ⟹ touches (x0 as s) (blockL_abs enc0 as s j)"
+  have Lcov: "\<And>j. j < length (enumL as s kk) \<Longrightarrow> touches (x0 as s) (blockL_abs enc0 as s j)"
     using Lcov_ALL by blast
-  have Rcov: "⋀j. j < length (enumR as s kk) ⟹ touches (x0 as s) (blockR_abs enc0 as s kk j)"
+  have Rcov: "\<And>j. j < length (enumR as s kk) \<Longrightarrow> touches (x0 as s) (blockR_abs enc0 as s kk j)"
     using Rcov_ALL by blast
 
   define x0 where "x0 = enc as s kk"
@@ -2763,90 +2894,90 @@ proof -
   define IR where "IR = {0..<length (enumR as s kk)}"
 
   (* pick one read index from each touched absolute block *)
-  define pickL where "pickL j = (SOME i. i ∈ R0 ∧ i ∈ blockL_abs enc0 as s j)" for j
-  define pickR where "pickR j = (SOME i. i ∈ R0 ∧ i ∈ blockR_abs enc0 as s kk j)" for j
+  define pickL where "pickL j = (SOME i. i \<in> R0 \<and> i \<in> blockL_abs enc0 as s j)" for j
+  define pickR where "pickR j = (SOME i. i \<in> R0 \<and> i \<in> blockR_abs enc0 as s kk j)" for j
 
  (* existence: each touched block contributes one read index *)
   have exL:
-    "⋀j. j ∈ IL ⟹ ∃i. i ∈ R0 ∧ i ∈ blockL_abs enc0 as s j"
+    "\<And>j. j \<in> IL \<Longrightarrow> \<exists>i. i \<in> R0 \<and> i \<in> blockL_abs enc0 as s j"
   proof -
-    fix j assume jIL: "j ∈ IL"
+    fix j assume jIL: "j \<in> IL"
     have jlt: "j < length (enumL as s kk)" using IL_def jIL by simp
     from Lcov[OF jlt] obtain i where
-      i1: "i ∈ Base.read0 M x0" and i2: "i ∈ blockL_abs enc0 as s j"
+      i1: "i \<in> Base.read0 M x0" and i2: "i \<in> blockL_abs enc0 as s j"
       using touches_def x0_def by blast
-    show "∃i. i ∈ R0 ∧ i ∈ blockL_abs enc0 as s j"
+    show "\<exists>i. i \<in> R0 \<and> i \<in> blockL_abs enc0 as s j"
       by (intro exI[of _ i]) (simp add: R0_def i1 i2)
   qed
 
   have exR:
-    "⋀j. j ∈ IR ⟹ ∃i. i ∈ R0 ∧ i ∈ blockR_abs enc0 as s kk j"
+    "\<And>j. j \<in> IR \<Longrightarrow> \<exists>i. i \<in> R0 \<and> i \<in> blockR_abs enc0 as s kk j"
   proof -
-    fix j assume jIR: "j ∈ IR"
+    fix j assume jIR: "j \<in> IR"
     have jlt: "j < length (enumR as s kk)" using IR_def jIR by simp
     from Rcov[OF jlt] obtain i where
-      i1: "i ∈ Base.read0 M x0" and i2: "i ∈ blockR_abs enc0 as s kk j"
+      i1: "i \<in> Base.read0 M x0" and i2: "i \<in> blockR_abs enc0 as s kk j"
       using touches_def x0_def by blast
-    show "∃i. i ∈ R0 ∧ i ∈ blockR_abs enc0 as s kk j"
+    show "\<exists>i. i \<in> R0 \<and> i \<in> blockR_abs enc0 as s kk j"
       by (intro exI[of _ i]) (simp add: R0_def i1 i2)
   qed
 
   (* witnesses belong to R0 and their blocks *)
   have pickL_in:
-    "⋀j. j ∈ IL ⟹ pickL j ∈ R0 ∧ pickL j ∈ blockL_abs enc0 as s j"
+    "\<And>j. j \<in> IL \<Longrightarrow> pickL j \<in> R0 \<and> pickL j \<in> blockL_abs enc0 as s j"
   proof -
-    fix j assume jIL: "j ∈ IL"
+    fix j assume jIL: "j \<in> IL"
     from exL[OF jIL]
-    show "pickL j ∈ R0 ∧ pickL j ∈ blockL_abs enc0 as s j"
+    show "pickL j \<in> R0 \<and> pickL j \<in> blockL_abs enc0 as s j"
       unfolding pickL_def by (rule someI_ex)
   qed
 
   have pickR_in:
-    "⋀j. j ∈ IR ⟹ pickR j ∈ R0 ∧ pickR j ∈ blockR_abs enc0 as s kk j"
+    "\<And>j. j \<in> IR \<Longrightarrow> pickR j \<in> R0 \<and> pickR j \<in> blockR_abs enc0 as s kk j"
   proof -
-    fix j assume jIR: "j ∈ IR"
+    fix j assume jIR: "j \<in> IR"
     from exR[OF jIR]
-    show "pickR j ∈ R0 ∧ pickR j ∈ blockR_abs enc0 as s kk j"
+    show "pickR j \<in> R0 \<and> pickR j \<in> blockR_abs enc0 as s kk j"
       unfolding pickR_def by (rule someI_ex)
   qed
 
   (* images are subsets of R0 *)
-  have subL: "pickL ` IL ⊆ R0"
+  have subL: "pickL ` IL \<subseteq> R0"
   proof
-    fix i assume "i ∈ pickL ` IL"
-    then obtain j where jIL: "j ∈ IL" and i_eq: "i = pickL j" by auto
-    from pickL_in[OF jIL] have "pickL j ∈ R0" by blast
-    thus "i ∈ R0" by (simp add: i_eq)
+    fix i assume "i \<in> pickL ` IL"
+    then obtain j where jIL: "j \<in> IL" and i_eq: "i = pickL j" by auto
+    from pickL_in[OF jIL] have "pickL j \<in> R0" by blast
+    thus "i \<in> R0" by (simp add: i_eq)
   qed
 
-  have subR: "pickR ` IR ⊆ R0"
+  have subR: "pickR ` IR \<subseteq> R0"
   proof
-    fix i assume "i ∈ pickR ` IR"
-    then obtain j where jIR: "j ∈ IR" and i_eq: "i = pickR j" by auto
-    from pickR_in[OF jIR] have "pickR j ∈ R0" by blast
-    thus "i ∈ R0" by (simp add: i_eq)
+    fix i assume "i \<in> pickR ` IR"
+    then obtain j where jIR: "j \<in> IR" and i_eq: "i = pickR j" by auto
+    from pickR_in[OF jIR] have "pickR j \<in> R0" by blast
+    thus "i \<in> R0" by (simp add: i_eq)
   qed
 
-  have union_sub: "pickL ` IL ∪ pickR ` IR ⊆ R0"
+  have union_sub: "pickL ` IL \<union> pickR ` IR \<subseteq> R0"
     using subL subR by auto
 
   (* injectivity inside L and inside R, by disjoint absolute blocks *)
   have injL: "inj_on pickL IL"
   proof (rule inj_onI)
-    fix j1 j2 assume j1: "j1 ∈ IL" and j2: "j2 ∈ IL" and eq: "pickL j1 = pickL j2"
-    obtain i1 where i1: "i1 ∈ R0 ∧ i1 ∈ blockL_abs enc0 as s j1" using exL[OF j1] by blast
-    obtain i2 where i2: "i2 ∈ R0 ∧ i2 ∈ blockL_abs enc0 as s j2" using exL[OF j2] by blast
-    have in1: "pickL j1 ∈ blockL_abs enc0 as s j1"
-      using ‹pickL ≡ λj. SOME i. i ∈ R0 ∧ i ∈ blockL_abs enc0 as s j› j1 pickL_in by auto
-    have in2: "pickL j2 ∈ blockL_abs enc0 as s j2"
-      using ‹pickL ≡ λj. SOME i. i ∈ R0 ∧ i ∈ blockL_abs enc0 as s j› j2 pickL_in by auto
+    fix j1 j2 assume j1: "j1 \<in> IL" and j2: "j2 \<in> IL" and eq: "pickL j1 = pickL j2"
+    obtain i1 where i1: "i1 \<in> R0 \<and> i1 \<in> blockL_abs enc0 as s j1" using exL[OF j1] by blast
+    obtain i2 where i2: "i2 \<in> R0 \<and> i2 \<in> blockL_abs enc0 as s j2" using exL[OF j2] by blast
+    have in1: "pickL j1 \<in> blockL_abs enc0 as s j1"
+      using \<open>pickL \<equiv> \<lambda>j. SOME i. i \<in> R0 \<and> i \<in> blockL_abs enc0 as s j\<close> j1 pickL_in by auto
+    have in2: "pickL j2 \<in> blockL_abs enc0 as s j2"
+      using \<open>pickL \<equiv> \<lambda>j. SOME i. i \<in> R0 \<and> i \<in> blockL_abs enc0 as s j\<close> j2 pickL_in by auto
     have inter_nonempty:
-      "blockL_abs enc0 as s j1 ∩ blockL_abs enc0 as s j2 ≠ {}"
+      "blockL_abs enc0 as s j1 \<inter> blockL_abs enc0 as s j2 \<noteq> {}"
       using eq in1 in2 by auto
     show "j1 = j2"
     proof (rule ccontr)
-      assume "j1 ≠ j2"
-      hence "blockL_abs enc0 as s j1 ∩ blockL_abs enc0 as s j2 = {}"
+      assume "j1 \<noteq> j2"
+      hence "blockL_abs enc0 as s j1 \<inter> blockL_abs enc0 as s j2 = {}"
         by (rule blockL_abs_disjoint)
       with inter_nonempty show False by contradiction
     qed
@@ -2854,41 +2985,41 @@ proof -
 
   have injR: "inj_on pickR IR"
   proof (rule inj_onI)
-    fix j1 j2 assume j1: "j1 ∈ IR" and j2: "j2 ∈ IR" and eq: "pickR j1 = pickR j2"
-    obtain i1 where i1: "i1 ∈ R0 ∧ i1 ∈ blockR_abs enc0 as s kk j1" using exR[OF j1] by blast
-    obtain i2 where i2: "i2 ∈ R0 ∧ i2 ∈ blockR_abs enc0 as s kk j2" using exR[OF j2] by blast
-    have in1: "pickR j1 ∈ blockR_abs enc0 as s kk j1"
-      using ‹pickR ≡ λj. SOME i. i ∈ R0 ∧ i ∈ blockR_abs enc0 as s kk j› j1 pickR_in by blast
-    have in2: "pickR j2 ∈ blockR_abs enc0 as s kk j2"
-      using ‹pickR ≡ λj. SOME i. i ∈ R0 ∧ i ∈ blockR_abs enc0 as s kk j› j2 pickR_in by blast
+    fix j1 j2 assume j1: "j1 \<in> IR" and j2: "j2 \<in> IR" and eq: "pickR j1 = pickR j2"
+    obtain i1 where i1: "i1 \<in> R0 \<and> i1 \<in> blockR_abs enc0 as s kk j1" using exR[OF j1] by blast
+    obtain i2 where i2: "i2 \<in> R0 \<and> i2 \<in> blockR_abs enc0 as s kk j2" using exR[OF j2] by blast
+    have in1: "pickR j1 \<in> blockR_abs enc0 as s kk j1"
+      using \<open>pickR \<equiv> \<lambda>j. SOME i. i \<in> R0 \<and> i \<in> blockR_abs enc0 as s kk j\<close> j1 pickR_in by blast
+    have in2: "pickR j2 \<in> blockR_abs enc0 as s kk j2"
+      using \<open>pickR \<equiv> \<lambda>j. SOME i. i \<in> R0 \<and> i \<in> blockR_abs enc0 as s kk j\<close> j2 pickR_in by blast
     have inter_nonempty:
-      "blockR_abs enc0 as s kk j1 ∩ blockR_abs enc0 as s kk j2 ≠ {}"
+      "blockR_abs enc0 as s kk j1 \<inter> blockR_abs enc0 as s kk j2 \<noteq> {}"
       using eq in1 in2 by auto
     show "j1 = j2"
     proof (rule ccontr)
-      assume "j1 ≠ j2"
-      hence "blockR_abs enc0 as s kk j1 ∩ blockR_abs enc0 as s kk j2 = {}"
+      assume "j1 \<noteq> j2"
+      hence "blockR_abs enc0 as s kk j1 \<inter> blockR_abs enc0 as s kk j2 = {}"
         by (rule blockR_abs_disjoint)
       with inter_nonempty show False by contradiction
     qed
   qed
 
   (* images are disjoint across L and R *)
-  have disj_images: "(pickL ` IL) ∩ (pickR ` IR) = {}"
+  have disj_images: "(pickL ` IL) \<inter> (pickR ` IR) = {}"
   proof
-    show "(pickL ` IL) ∩ (pickR ` IR) ⊆ {}"
+    show "(pickL ` IL) \<inter> (pickR ` IR) \<subseteq> {}"
     proof
-      fix i assume iin: "i ∈ (pickL ` IL) ∩ (pickR ` IR)"
-      then obtain jL where jL: "jL ∈ IL" and iL: "i = pickL jL" by blast
-      from iin obtain jR where jR: "jR ∈ IR" and iR: "i = pickR jR" by blast
-      have inL: "i ∈ blockL_abs enc0 as s jL"
+      fix i assume iin: "i \<in> (pickL ` IL) \<inter> (pickR ` IR)"
+      then obtain jL where jL: "jL \<in> IL" and iL: "i = pickL jL" by blast
+      from iin obtain jR where jR: "jR \<in> IR" and iR: "i = pickR jR" by blast
+      have inL: "i \<in> blockL_abs enc0 as s jL"
         using iL pickL_in[OF jL] by auto
-      have inR: "i ∈ blockR_abs enc0 as s kk jR"
+      have inR: "i \<in> blockR_abs enc0 as s kk jR"
         using iR pickR_in[OF jR] by auto
       have jL_lt: "jL < length (enumL as s kk)" using IL_def jL by auto
-      have disj: "blockL_abs enc0 as s jL ∩ blockR_abs enc0 as s kk jR = {}"
+      have disj: "blockL_abs enc0 as s jL \<inter> blockR_abs enc0 as s kk jR = {}"
         by (rule blockL_abs_blockR_abs_disjoint[OF jL_lt])
-      from inL inR disj show "i ∈ {}" by auto
+      from inL inR disj show "i \<in> {}" by auto
     qed
   qed simp
 
@@ -2897,18 +3028,18 @@ proof -
   have fin_imgL: "finite (pickL ` IL)" by (intro finite_imageI) (simp add: IL_def)
   have fin_imgR: "finite (pickR ` IR)" by (intro finite_imageI) (simp add: IR_def)
 
-  have card_lower: "card (pickL ` IL ∪ pickR ` IR) ≤ card R0"
+  have card_lower: "card (pickL ` IL \<union> pickR ` IR) \<le> card R0"
     by (rule card_mono[OF fin_R0 union_sub])
 
   have card_union:
-    "card (pickL ` IL ∪ pickR ` IR) = card (pickL ` IL) + card (pickR ` IR)"
+    "card (pickL ` IL \<union> pickR ` IR) = card (pickL ` IL) + card (pickR ` IR)"
     by (subst card_Un_disjoint) (use disj_images fin_imgL fin_imgR in auto)
 
   have inj_cardL: "card (pickL ` IL) = card IL" by (rule card_image[OF injL])
   have inj_cardR: "card (pickR ` IR) = card IR" by (rule card_image[OF injR])
 
   from card_lower card_union inj_cardL inj_cardR
-  have A: "card IL + card IR ≤ card R0" by simp
+  have A: "card IL + card IR \<le> card R0" by simp
 
   have card_IL: "card IL = card (LHS (e_k as s kk) n)"
     by (simp add: IL_def enumL_def n_def)
@@ -2916,13 +3047,13 @@ proof -
     by (simp add: IR_def enumR_def n_def)
 
   have B:
-   "card (LHS (e_k as s kk) n) + card (RHS (e_k as s kk) n) ≤ card R0"
+   "card (LHS (e_k as s kk) n) + card (RHS (e_k as s kk) n) \<le> card R0"
     using A by (simp add: card_IL card_IR)
 
   (* final sandwich with steps *)
-  have "card R0 ≤ steps M x0"
+  have "card R0 \<le> steps M x0"
     by (simp add: R0_def Base.card_read0_le_steps)
-  from B this have "card (LHS (e_k as s kk) n) + card (RHS (e_k as s kk) n) ≤ steps M x0"
+  from B this have "card (LHS (e_k as s kk) n) + card (RHS (e_k as s kk) n) \<le> steps M x0"
     by (rule le_trans)
   thus ?thesis
     unfolding x0_def by blast
@@ -2932,33 +3063,33 @@ qed
 lemma coverage_blocks_from_distinct:
   assumes n_def: "n = length as"
       and distinct: "distinct_subset_sums as"
-      and kk_le:     "kk ≤ n"
-      and kk_pos:    "1 ≤ kk"   (* keep if you really need nontrivial split *)
+      and kk_le:     "kk \<le> n"
+      and kk_pos:    "1 \<le> kk"   (* keep if you really need nontrivial split *)
   shows
-   "(∀j<length (enumL as s kk). touches (enc as s kk) (blockL_abs enc0 as s j)) ∧
-    (∀j<length (enumR as s kk). touches (enc as s kk) (blockR_abs enc0 as s kk j))"
+   "(\<forall>j<length (enumL as s kk). touches (enc as s kk) (blockL_abs enc0 as s j)) \<and>
+    (\<forall>j<length (enumR as s kk). touches (enc as s kk) (blockR_abs enc0 as s kk j))"
 proof -
   (* discharge the eight premises ONCE here; replace sorry by your lemmas *)
-  have L2:   "2 ≤ length (enumL as s kk)" sorry
-  have hitL: "∃v∈set (enumL as s kk). v ∈ set (enumR as s kk)" sorry
-  have missL:"∃v∈set (enumL as s kk). v ∉ set (enumR as s kk)" sorry
+  have L2:   "2 \<le> length (enumL as s kk)" sorry
+  have hitL: "\<exists>v\<in>set (enumL as s kk). v \<in> set (enumR as s kk)" sorry
+  have missL:"\<exists>v\<in>set (enumL as s kk). v \<notin> set (enumR as s kk)" sorry
   have base_only_L:
-    "⋀j. Good as s ((!) (enc as s kk)) ((!) (enc as s kk)) ⟹
-         (∀j'<length (enumL as s kk). j' ≠ j ⟶
-            Lval_at as s ((!) (enc as s kk)) j' ∉ set (enumR as s kk))" sorry
+    "\<And>j. Good as s ((!) (enc as s kk)) ((!) (enc as s kk)) \<Longrightarrow>
+         (\<forall>j'<length (enumL as s kk). j' \<noteq> j \<longrightarrow>
+            Lval_at as s ((!) (enc as s kk)) j' \<notin> set (enumR as s kk))" sorry
 
-  have R2:   "2 ≤ length (enumR as s kk)" sorry
-  have hitR: "∃v∈set (enumR as s kk). v ∈ set (enumL as s kk)" sorry
-  have missR:"∃v∈set (enumR as s kk). v ∉ set (enumL as s kk)" sorry
+  have R2:   "2 \<le> length (enumR as s kk)" sorry
+  have hitR: "\<exists>v\<in>set (enumR as s kk). v \<in> set (enumL as s kk)" sorry
+  have missR:"\<exists>v\<in>set (enumR as s kk). v \<notin> set (enumL as s kk)" sorry
   have base_only_R:
-    "⋀j. Good as s ((!) (x0 as s)) ((!) (x0 as s)) ⟹
-         (∀j'<length (enumR as s kk). j' ≠ j ⟶
-            Rval_at as s ((!) (x0 as s)) j' ∉ set (enumL as s kk))" sorry
+    "\<And>j. Good as s ((!) (x0 as s)) ((!) (x0 as s)) \<Longrightarrow>
+         (\<forall>j'<length (enumR as s kk). j' \<noteq> j \<longrightarrow>
+            Rval_at as s ((!) (x0 as s)) j' \<notin> set (enumL as s kk))" sorry
 
   have cov_enc:
-    "(∀j<length (enumL as s kk).
-        touches (enc as s kk) (blockL_abs enc0 as s j)) ∧
-     (∀j<length (enumR as s kk).
+    "(\<forall>j<length (enumL as s kk).
+        touches (enc as s kk) (blockL_abs enc0 as s j)) \<and>
+     (\<forall>j<length (enumR as s kk).
         touches (enc as s kk) (blockR_abs enc0 as s kk j))"
     by (rule coverage_blocks[
           OF n_def distinct
@@ -2971,21 +3102,21 @@ qed
 lemma steps_lower_bound:
   assumes n_def: "n = length as"
       and distinct: "distinct_subset_sums as"
-      and kk_le: "kk ≤ n"
-      and kk_pos: "1 ≤ kk"   (* drop if not needed *)
+      and kk_le: "kk \<le> n"
+      and kk_pos: "1 \<le> kk"   (* drop if not needed *)
   shows "steps M (enc as s kk)
-         ≥ card (LHS (e_k as s kk) n) + card (RHS (e_k as s kk) n)"
+         \<ge> card (LHS (e_k as s kk) n) + card (RHS (e_k as s kk) n)"
 proof -
   obtain Lcov_ALL Rcov_ALL where
-    Lcov_ALL: "∀j<length (enumL as s kk).
+    Lcov_ALL: "\<forall>j<length (enumL as s kk).
                  touches (enc as s kk) (blockL_abs enc0 as s j)" and
-    Rcov_ALL: "∀j<length (enumR as s kk).
+    Rcov_ALL: "\<forall>j<length (enumR as s kk).
                  touches (enc as s kk) (blockR_abs enc0 as s kk j)"
     using coverage_blocks_from_distinct[OF n_def distinct kk_le kk_pos] by blast
 
   (* From here: paste your existing counting proof unchanged,
      but use Lcov_ALL / Rcov_ALL in place of the old premises. *)
-  (* ... pickL/pickR definitions, show images ⊆ read0, disjointness,
+  (* ... pickL/pickR definitions, show images \<subseteq> read0, disjointness,
          card_Un_disjoint, card_image via inj_on, etc ...
      Exactly as you already had in your previous working proof. *)
 
